ocaml/Mininet.ml
@@ -1,0 +1,19 @@
+open Lexing
+open Printf
+
+let string_of_position p =
+  Format.sprintf "%s:%d:%d" p.pos_fname p.pos_lnum (p.pos_cnum - p.pos_bol)
+
+let parse_from_chan cin name =
+  let lexbuf = Lexing.from_channel cin in
+    try
+      lexbuf.lex_curr_p <- { lexbuf.lex_curr_p with pos_fname = name };
+      MininetParser.program MininetLexer.token lexbuf
+    with
+      |  Failure "lexing: empty token" ->
+           failwith (sprintf "lexical error at %s"
+                       (string_of_position lexbuf.lex_curr_p))
+      | MininetParser.Error ->
+           failwith (sprintf "parse error at %s; unexpected token %s"
+                       (string_of_position lexbuf.lex_curr_p)
+                       (lexeme lexbuf))
