ocaml/Mininet.mli
@@ -1,0 +1,3 @@
+open MininetTypes
+      
+val parse_from_chan : in_channel -> string -> (node * portId * node) list
