ocaml/MininetTypes.ml
@@ -1,0 +1,7 @@
+type switchId = Int64.t
+type hostAddr = Int64.t
+type portId = int
+
+type node =
+  | Host of hostAddr
+  | Switch of switchId
