ocaml/PolicyGenerator.ml
@@ -1,0 +1,106 @@
+module type PARAM = sig
+
+  type node
+  type edge_label
+
+end
+
+module type DIRECTED_GRAPH = sig
+ 
+  type node
+  type edge_label
+ 
+  type t
+
+  val empty : unit -> t
+
+  val add_edge : t -> node -> edge_label -> node -> unit
+
+  val all_nodes : t -> node list
+
+  val shortest_path : t -> node -> node -> node list
+
+end 
+
+
+let singleton_hashtbl k v =
+  let h = Hashtbl.create 100 in
+  Hashtbl.add h k v;
+  h
+
+module Make (Param : PARAM) : DIRECTED_GRAPH = struct
+
+  type node = Param.node
+
+  type edge_label = Param.edge_label
+
+  (* Map from sources to a table of sinks and the edge label *)
+  type t = { 
+    graph : (node, (node, edge_label) Hashtbl.t) Hashtbl.t;
+    nodes : (node, unit) Hashtbl.t
+  }
+
+  let empty () : t = 
+    { graph = Hashtbl.create 100; nodes = Hashtbl.create 10 }
+
+  let add_edge (g : t) (s : node) (x : edge_label) (d : node) =
+    begin
+      try 
+        let s_edges_out = Hashtbl.find g.graph s in
+        if Hashtbl.mem s_edges_out d then
+          failwith "edge exists"
+        else
+            Hashtbl.add s_edges_out d x
+      with
+        | Not_found ->
+          Hashtbl.add g.graph s (singleton_hashtbl d x)
+    end;
+    (if not (Hashtbl.mem g.nodes s) then
+      Hashtbl.add g.nodes s ());
+    (if not (Hashtbl.mem g.nodes d) then
+      Hashtbl.add g.nodes d ())
+
+  let all_nodes g =
+    Hashtbl.fold (fun n _ lst -> n :: lst) g.nodes []
+
+  let succs g s =
+    try
+      let succ_tbl = Hashtbl.find g.graph s in
+      Hashtbl.fold (fun vx edge lst -> (vx :: lst))  succ_tbl []
+    with
+        Not_found -> failwith "node does not exist in succs"
+
+  let shortest_path g s d = 
+    let rec loop fringe = 
+      match fringe with
+        | [] -> []
+        | [] :: _ -> failwith "impossible case during BFS"
+        | (x :: xs) :: rest ->
+          let nexts = succs g x in
+          if List.mem s nexts then
+            loop rest (* avoid silly cycles *)
+          else if List.mem d nexts then
+            (d :: x :: xs)
+          else
+            loop (fringe @ List.map (fun y -> y :: x :: xs) nexts) in
+    if s = d then
+      [s]
+    else
+      loop (List.map (fun x -> [x]) (succs g s))
+
+
+end
+
+
+
+
+module Params = struct
+
+  type node = MininetTypes.node
+
+  type edge_label = int (* egress port, bogus for hosts *)
+
+end
+
+module PolicyGraph = Make (Params)
+
