ocaml/VerifiedNetCore.ml
@@ -1,0 +1,137 @@
+open ControllerInterface
+open MessagesDef
+open Packet
+open Platform
+open Printf
+open NetCoreSyntax
+
+module CoqCtrl = FwOFSimpleExtractableController
+
+module type POLICY = sig
+  val policy : policy
+  (* Necessary due to static compilation in FwOF. *)
+  val switches : switchId list
+end
+
+(* Topology is not relevant for execution, only the proof. See the note below.
+*)
+module MakePolTopo (Policy : POLICY) : CoqCtrl.POLICY_AND_TOPOLOGY = struct
+
+  (* Note: this is not relevant for execution. It is only needed for
+     verification. The signatures in Coq (FwOFSignatures.v) should be better
+     factored so that this cruft is not neeeded. *)
+  let topo _ = None  
+
+  let handlers = Hashtbl.create 0
+
+  let pol = desugar_policy Policy.policy handlers
+
+  let get_pkt out = 
+    let open NetCoreEval in
+    match out with
+      | OutPkt (sw,PhysicalPort pt, pk, Datatypes.Coq_inl buf) ->
+        Some (pt, (pk, buf))
+      | _ -> None
+        
+
+  let abst_func sw pt (pk,buf) = 
+    let open NetCoreEval in
+    Types.filter_map get_pkt (classify pol (InPkt (sw,pt,pk, Some buf)))
+
+end
+
+
+module Make (Platform : PLATFORM) (Policy : POLICY) = struct
+
+  module Controller = CoqCtrl.Make (MakePolTopo (Policy))
+
+  type state = Controller.state
+
+  let init_packet_out () = {
+    Controller.pktsToSend = []; 
+    Controller.switchStates = []
+  }
+
+  let pending_switches : (switchId, bool) Hashtbl.t = Hashtbl.create 100
+
+  let rec accept_switches () = 
+    Lwt.bind (Platform.accept_switch ())
+      (fun feats -> 
+        (if Hashtbl.mem pending_switches feats.switch_id then
+          Hashtbl.remove pending_switches feats.switch_id
+        else
+          eprintf "[VerifiedNetCore.ml]: unexpected connection from %Ld"
+            feats.switch_id);
+        if Hashtbl.length pending_switches > 0 then
+          begin
+            eprintf "[VerifiedNetCore.ml]: waiting for next switch.";
+            accept_switches ()
+          end
+        else
+          Lwt.return ())
+
+  let start (init_state : state) = 
+    List.iter (fun sw -> Hashtbl.add pending_switches sw true) Policy.switches;
+    accept_switches ()
+
+end
+
+(*
+  (Handlers : HANDLERS) = struct
+
+  (* The monad is written in OCaml *)
+  module NetCoreMonad = MakeNetCoreMonad (Platform) (Handlers)
+  (* The controller is written in Coq *)
+  module Controller = NetCoreController.Make (NetCoreMonad)
+
+  let start_controller policy_stream =
+    let init_state = { 
+      NetCoreController.policy = drop_all_packets; 
+      NetCoreController.switches = []
+    } in
+    let policy_stream = Lwt_stream.map (fun v -> Policy v) policy_stream in
+    let event_stream = Lwt_stream.map (fun v -> Event v)
+      (Lwt_channel.to_stream NetCoreMonad.events) in
+    let event_or_policy_stream = Lwt_stream.choose 
+      [ event_stream ; policy_stream ] in
+    let body = fun state ->
+      Lwt.bind (Lwt_stream.next event_or_policy_stream)
+        (fun v -> match v with
+          | Event ev -> 
+            printf "[NetCore.ml] new event, calling handler\n%!";
+            Controller.handle_event ev state
+          | Policy pol ->
+            printf "[NetCore.ml] new policy\n%!";
+            Controller.set_policy pol state) in
+    let main = NetCoreMonad.forever body in
+    NetCoreMonad.run init_state main
+
+end
+
+module Make (Policy : POLICY) (Platform : PLATFORM) = struct
+
+  let get_pkt_handlers : (int, get_packet_handler) Hashtbl.t = Hashtbl.create 0
+
+  let start () 
+
+    Hashtbl.create 200
+
+  module Handlers : HANDLERS = struct
+      
+    let get_packet_handler queryId switchId portId packet = 
+      printf "[NetCore.ml] Got packet from %Ld\n" switchId;
+        (Hashtbl.find get_pkt_handlers queryId) switchId portId packet
+  end
+
+  module Controller = MakeDynamic (Platform) (Handlers)
+
+  let start_controller (pol : policy Lwt_stream.t) : unit Lwt.t = 
+    Controller.start_controller
+      (Lwt_stream.map 
+         (fun pol -> 
+           printf "[NetCore.ml] got a new policy%!\n";
+           NetCoreSyntax.desugar_policy pol get_pkt_handlers)
+         pol)
+
+end
+*)
