ocaml/VerifiedNetCore.mli
@@ -1,0 +1,22 @@
+open ControllerInterface
+open MessagesDef
+open Packet
+open Platform
+open Printf
+open NetCoreSyntax
+
+module type POLICY = sig
+  val policy : policy
+  (* Necessary due to static compilation in FwOF. *)
+  val switches : switchId list
+end
+
+
+module Make (Platform : PLATFORM) (Policy : POLICY) : sig
+
+  type state
+
+  val init_packet_out : unit -> state
+  val start : state -> unit Lwt.t
+
+end
