coq/FwOF/FwOFMachine.v
@@ -38,10 +38,7 @@ Module Make (Atoms_ : ATOMS) <: MACHINE.
       switchId_le (swId sw1) (swId sw2) ->
       switch_le sw1 sw2.
 
-  Instance TotalOrder_switch : TotalOrder switch_le.
-  Proof with auto.
-    split.
-  Admitted.
+  Axiom Instance TotalOrder_switch : TotalOrder switch_le.
   
   Record dataLink := DataLink {
     src : switchId * portId;
@@ -202,6 +199,7 @@ Module Make (Atoms_ : ATOMS) <: MACHINE.
         obs
         (State (({|sw0|}) <+> sws) links (ofLinks ++ of0 :: ofLinks0) ctrl)).
 
+
   Definition swPtPks : Type :=
     bag (PairOrdering (PairOrdering switchId_le portId_le)
                       packet_le).
@@ -240,281 +238,31 @@ Module Make (Atoms_ : ATOMS) <: MACHINE.
       unions (map (select_packet_in sw) (map (PacketIn pt) packetIns)) =
       unions (map (transfer sw) (abst_func sw pt pk)).
 
-  Section FlowModSafety.
+  Inductive NotFlowMod : fromController -> Prop :=
+  | NotFlowMod_BarrierRequest : forall n, NotFlowMod (BarrierRequest n)
+  | NotFlowMod_PacketOut : forall pt pk, NotFlowMod (PacketOut pt pk).
 
-    Inductive Endpoint : Type :=
-    | Endpoint_NoBarrier : flowTable -> Endpoint
-    | Endpoint_Barrier : flowTable -> Endpoint.
-
-    Definition table_at_endpoint (ep : Endpoint) :=
-      match ep with
-        | Endpoint_NoBarrier tbl => tbl
-        | Endpoint_Barrier tbl => tbl
-      end.
-
-    Inductive SafeWire : switchId -> 
-                    Endpoint -> 
-                    list fromController ->
-                    Endpoint -> Prop :=
-    | SafeWire_nil : forall swId ep,
-      FlowTableSafe swId (table_at_endpoint ep) ->
-      SafeWire swId ep nil ep
-    | SafeWire_PktOut : forall swId pt pk ctrlEp ctrlm swEp,
-      SafeWire swId ctrlEp ctrlm swEp ->
-      SafeWire swId ctrlEp (PacketOut pt pk :: ctrlm) swEp
-    | SafeWire_BarrierRequest : forall swId n ctrlEp ctrlm swEp,
-      SafeWire swId ctrlEp ctrlm swEp ->
-      SafeWire swId (Endpoint_Barrier (table_at_endpoint ctrlEp))
-                    (BarrierRequest n :: ctrlm)
-                    swEp
-    | SafeWire_FlowMod : forall swId f tbl ctrlm swEp,
-      FlowTableSafe swId (modify_flow_table f tbl) ->
-      SafeWire swId (Endpoint_Barrier tbl) ctrlm swEp ->
-      SafeWire swId (Endpoint_NoBarrier (modify_flow_table f tbl))
-          (FlowMod f :: ctrlm) swEp.
-
-    Inductive NotFlowMod : fromController -> Prop :=
-    | NotFlowMod_BarrierRequest : forall n, NotFlowMod (BarrierRequest n)
-    | NotFlowMod_PacketOut : forall pt pk, NotFlowMod (PacketOut pt pk).
-
-    Inductive SwitchEP : switch -> Endpoint -> Prop :=
-    | NoFlowModsInBuffer : forall swId pts tbl inp outp ctrlm switchm swEp,
+  Inductive FlowModSafe : switchId -> flowTable -> bag fromController_le -> Prop :=
+  | NoFlowModsInBuffer : forall swId tbl ctrlm,
       (forall msg, In msg (to_list ctrlm) -> NotFlowMod msg) ->
-      table_at_endpoint swEp = tbl ->
-      SwitchEP
-        (Switch swId pts tbl inp outp ctrlm switchm)
-        swEp
-    | OneFlowModInBuffer : forall swId pts tbl inp outp ctrlm ctrlm0 switchm f,
-      (forall msg, In msg (to_list ctrlm0) -> NotFlowMod msg) ->
-      ctrlm = ({|FlowMod f|} <+> ctrlm0) ->
+      FlowTableSafe swId tbl ->
+      FlowModSafe swId tbl ctrlm
+  | OneFlowModsInBuffer : forall swId tbl ctrlm f,
+      (forall msg, In msg (to_list ctrlm) -> NotFlowMod msg) ->
+      FlowTableSafe swId tbl ->
       FlowTableSafe swId (modify_flow_table f tbl) ->
-      SwitchEP (Switch swId pts tbl inp outp ctrlm switchm)
-               (Endpoint_NoBarrier (modify_flow_table f tbl)).
+      FlowModSafe swId tbl (({|FlowMod f|}) <+> ctrlm).
+ 
+  Definition FlowTablesSafe (sws : bag switch_le) : Prop :=
+    forall swId pts tbl inp outp ctrlm switchm,
+      In (Switch swId pts tbl inp outp ctrlm switchm) (to_list sws) ->
+      FlowModSafe swId tbl ctrlm.
 
-    (** "FMS" is short for "flow mod safety". *)
-    Inductive FMS : switch -> openFlowLink -> Prop := 
-    | MkFMS : forall swId pts tbl inp outp ctrlm switchm ctrlmList 
-                     switchmList
-                     switchEp,
-      SwitchEP (Switch swId pts tbl inp outp ctrlm switchm) switchEp ->
-      (exists ctrlEp, SafeWire swId ctrlEp ctrlmList switchEp) ->
-      FMS 
-        (Switch swId pts tbl inp outp ctrlm switchm)
-        (OpenFlowLink swId switchmList ctrlmList).
-
-    Definition AllFMS (sws : bag switch_le) 
-                      (ofLinks : list openFlowLink) :=
-      forall sw,
-        In sw (to_list sws) ->
-        exists lnk, 
-          In lnk ofLinks /\
-          of_to lnk = swId sw /\
-          FMS sw lnk.
-
-
-    Hint Constructors Endpoint SafeWire NotFlowMod SwitchEP FMS.
-
-
-    Lemma FMS_untouched : forall swId0 pts0 tbl0 inp0 outp0 ctrlm0 switchm0
-      switchmLst0 ctrlmLst0 inp1 outp1 switchm1 switchmLst1,
-      FMS (Switch swId0 pts0 tbl0 inp0 outp0 ctrlm0 switchm0)
-          (OpenFlowLink swId0 switchmLst0 ctrlmLst0) ->
-      FMS (Switch swId0 pts0 tbl0 inp1 outp1 ctrlm0 switchm1)
-          (OpenFlowLink swId0 switchmLst1 ctrlmLst0).
-    Proof.
-      intros.
-      inversion H; inversion H2; subst; eauto.
-    Qed.
-
-
-    Lemma SafeWire_dequeue_PacketOut : forall sw ctrlEp ctrlLst pt pk switchEp,
-      SafeWire sw ctrlEp (ctrlLst ++ [PacketOut pt pk]) switchEp ->
-      SafeWire sw ctrlEp (ctrlLst) switchEp.
-    Proof with auto.
-      intros.
-      generalize dependent ctrlEp.
-      induction ctrlLst; intros.
-      + simpl in H. inversion H. subst...
-      + inversion H; subst...
-    Qed.
-
-    Lemma SafeWire_dequeue_BarrierRequest : forall sw ctrlEp ctrlLst xid 
-      switchEp1,
-      SafeWire sw ctrlEp (ctrlLst ++ [BarrierRequest xid]) switchEp1 ->
-      exists switchEp2, SafeWire sw ctrlEp (ctrlLst) switchEp2 /\
-        table_at_endpoint switchEp2 = table_at_endpoint switchEp1.
-    Proof with eauto.
-      intros.
-      generalize dependent ctrlEp.
-      induction ctrlLst; intros.
-      + inversion H; subst.
-        inversion H5. subst.
-        exists (Endpoint_Barrier (table_at_endpoint switchEp1)).
-        split.
-        apply SafeWire_nil.
-        simpl...
-        simpl...
-      + simpl in H.
-        inversion H; subst.
-        * apply IHctrlLst in H5.
-          destruct H5 as [switchEp2 [HSafeWire HEpEq]].
-          exists switchEp2.
-          split; simpl...
-        * apply IHctrlLst in H5.
-          destruct H5 as [switchEp2 [HSafeWire HEpEq]].
-          exists switchEp2.
-          split; simpl...
-        * apply IHctrlLst in H6.
-          destruct H6 as [switchEp2 [HSafeWire HEpEq]].
-          exists switchEp2.
-          split; simpl...
-    Qed.
-
-    Lemma SafeWire_dequeue_safe : forall sw ctrlEp ctrlLst f switchEp,
-       SafeWire sw ctrlEp (ctrlLst ++ [FlowMod f]) switchEp ->
-       FlowTableSafe sw (modify_flow_table f (table_at_endpoint switchEp)).
-    Proof with auto.
-      intros.
-      generalize dependent ctrlEp.
-      { induction ctrlLst; intros.
-        + destruct switchEp.
-          simpl in H.
-          inversion H.
-          subst.
-          inversion H6.
-          simpl in H.
-          inversion H.
-          subst.
-          inversion H6.
-          subst.
-          simpl...
-        + simpl in *.
-          inversion H; subst.
-          - apply IHctrlLst in H5...
-          - apply IHctrlLst in H5...
-          - apply IHctrlLst in H6... }
-    Qed.
-
-    Lemma SafeWire_dequeue_FlowMod : forall sw ctrlEp ctrlLst f switchEp,
-       SafeWire sw ctrlEp (ctrlLst ++ [FlowMod f]) switchEp ->
-       SafeWire sw ctrlEp ctrlLst (Endpoint_NoBarrier (modify_flow_table f (table_at_endpoint switchEp))).
-    Proof with auto.
-      intros.
-      generalize dependent ctrlEp.
-      { induction ctrlLst; intros.
-        + destruct switchEp.
-          simpl in H.
-          inversion H.
-          subst.
-          inversion H6.
-          simpl in H.
-          inversion H.
-          subst.
-          inversion H6.
-          subst.
-          simpl...
-        + simpl in *.
-          inversion H; subst.
-          - apply IHctrlLst in H5...
-          - apply IHctrlLst in H5...
-          - apply IHctrlLst in H6... }
-    Qed.
-
-    Lemma SafeWire_fm_nb_false : forall sw ctrlEp ctrlLst f tbl,
-      SafeWire sw ctrlEp (ctrlLst ++ [FlowMod f]) (Endpoint_NoBarrier tbl) ->
-      False.
-    Proof with auto.
-      intros.
-      generalize dependent ctrlEp.
-      induction ctrlLst; intros.
-      + simpl in H. inversion H. subst. inversion H6.
-      + simpl in H.
-        inversion H; subst.
-        - apply IHctrlLst in H5...
-          - apply IHctrlLst in H5...
-          - apply IHctrlLst in H6...
-    Qed.
-
-    Lemma FMS_pop : forall sw pts tbl inp outp ctrlm switchm switchLst ctrlLst msg,
-      FMS  (Switch sw pts tbl inp outp ctrlm switchm) (OpenFlowLink sw switchLst (ctrlLst ++ [msg])) ->
-      FMS  (Switch sw pts tbl inp outp ({|msg|} <+> ctrlm) switchm) (OpenFlowLink sw switchLst ctrlLst).
-    Proof with eauto.
-      intros.
-      inversion H.
-      subst.
-      destruct H10 as [ctrlEp HSafeWire].
-      { destruct msg.
-        + apply MkFMS with (switchEp := switchEp).
-          * inversion H2; subst.
-            - apply NoFlowModsInBuffer...
-              intros.
-              apply Bag.in_union in H0.
-              simpl in H0.
-              destruct H0 as [[H0 | H0] | H0]...
-              destruct msg...
-              inversion H0.
-              inversion H0.
-            - apply OneFlowModInBuffer 
-                with (ctrlm0 := ({|PacketOut p p0|} <+> ctrlm2))...
-              intros.
-              apply Bag.in_union in H0.
-              simpl in H0.
-              destruct H0 as [[H0 | H0] | H0]...
-              destruct msg...
-              inversion H0.
-              inversion H0.
-              bag_perm 10.
-          * exists ctrlEp.
-            eapply SafeWire_dequeue_PacketOut.
-            exact HSafeWire.
-        + admit. (* strange case where barrier is added to switch. *)
-        + inversion H2; subst.
-          * apply MkFMS with (switchEp := (Endpoint_NoBarrier (modify_flow_table f (table_at_endpoint switchEp)))).
-            apply OneFlowModInBuffer with (ctrlm0 := ctrlm0)...
-            eapply SafeWire_dequeue_safe.
-            exact HSafeWire.
-            exists ctrlEp.
-            apply SafeWire_dequeue_FlowMod...
-         * contradiction (SafeWire_fm_nb_false _ _ HSafeWire).
-      }
-    Qed.
-
-    Lemma FMS_dequeue_pktOut : forall sw pts tbl inp outp ctrlm switchm switchLst ctrlLst pt pk,
-      FMS  (Switch sw pts tbl inp outp ({|PacketOut pt pk|} <+> ctrlm) switchm) (OpenFlowLink sw switchLst ctrlLst) ->
-      FMS  (Switch sw pts tbl inp ({|(pt,pk)|} <+> outp) ctrlm switchm) (OpenFlowLink sw switchLst ctrlLst).
-    Proof with eauto.
-      intros.
-      inversion H.
-      subst.
-      destruct H10 as [ctrlEp HSafeWire].
-      apply MkFMS with (switchEp := switchEp).
-      inversion H2; subst.
-      - apply NoFlowModsInBuffer...
-        intros.
-        apply H9.
-        apply Bag.in_union...
-      - assert (In (PacketOut pt pk) (to_list ctrlm2)) as J.
-        {      
-          assert (In (PacketOut pt pk) (to_list ({|FlowMod f|} <+> ctrlm2))).
-          { rewrite <- H10. apply Bag.in_union. left. simpl... }
-          apply Bag.in_union in H0.
-          destruct H0 as [[H0 | H0] | H0]...
-          inversion H0.
-          inversion H0. } 
-        apply Bag.in_split with (Order:=TotalOrder_fromController) in J.
-        destruct J as [ctrlm1 Heq].
-        subst.
-        apply OneFlowModInBuffer with
-          (ctrlm0 := ctrlm1)...
-        intros.
-        apply H9.
-        apply Bag.in_union. right...
-        apply (Bag.pop_union_l _ ({|PacketOut pt pk|})).
-        rewrite -> H10.
-        bag_perm 100. 
-      - exists ctrlEp...
-    Qed.
-
-  End FlowModSafety.
+  Definition SwitchesHaveOpenFlowLinks (sws : bag switch_le) ofLinks :=
+    forall sw,
+      In sw (to_list sws) ->
+      exists ofLink,
+        In ofLink ofLinks /\
+        swId sw = of_to ofLink.
 
 End Make.
