coq/FwOF/FwOFSimpleControllerLemmas.v
@@ -16,9 +16,7 @@ Local Open Scope bag_scope.
 
 Module MakeController (NetAndPol : NETWORK_AND_POLICY) <: ATOMS_AND_CONTROLLER.
   Module Import Atoms := FwOF.FwOFSimpleController.Make (NetAndPol).
-  Module Machine := FwOF.FwOFMachine.Make (Atoms).
-  Import Machine.
-
+  Module Import Machine := FwOF.FwOFMachine.Make (Atoms).
   Require Import Bag.Bag2.
 
   Inductive NotPacketOut : fromController -> Prop :=
@@ -27,23 +25,284 @@ Module MakeController (NetAndPol : NETWORK_AND_POLICY) <: ATOMS_AND_CONTROLLER.
   | FlowMod_NotPacketOut : forall fm,
       NotPacketOut (FlowMod fm).
 
-  Hint Constructors NotPacketOut.
+  Hint Constructors NotPacketOut NotFlowMod.
+
+
+  Inductive Endpoint : Type :=
+  | Endpoint_FlowMod : flowTable -> Endpoint
+  | Endpoint_Barrier : flowTable -> Endpoint.
+
+  Definition table_at_endpoint (ep : Endpoint) :=
+    match ep with
+      | Endpoint_FlowMod tbl => tbl
+      | Endpoint_Barrier tbl => tbl
+    end.
+
+
+  Inductive SafeWire : switchId -> 
+                    Endpoint -> 
+                    list fromController ->
+                    Endpoint -> Prop :=
+    | SafeWire_nil : forall swId ep,
+      FlowTableSafe swId (table_at_endpoint ep) ->
+      SafeWire swId ep nil ep
+    | SafeWire_PktOut : forall swId pt pk ctrlEp ctrlm swEp,
+      SafeWire swId ctrlEp ctrlm swEp ->
+      SafeWire swId ctrlEp (PacketOut pt pk :: ctrlm) swEp
+    | SafeWire_BarrierRequest : forall swId n ctrlEp ctrlm swEp,
+      SafeWire swId ctrlEp ctrlm swEp ->
+      SafeWire swId (Endpoint_Barrier (table_at_endpoint ctrlEp))
+                    (BarrierRequest n :: ctrlm)
+                    swEp
+    | SafeWire_FlowMod : forall swId f tbl ctrlm swEp,
+      FlowTableSafe swId (modify_flow_table f tbl) ->
+      SafeWire swId (Endpoint_Barrier tbl) ctrlm swEp ->
+      SafeWire swId (Endpoint_FlowMod (modify_flow_table f tbl))
+          (FlowMod f :: ctrlm) swEp.  
+
+
+  Inductive Barriered : switchId -> list fromController -> flowTable -> bag fromController_le -> Prop :=
+  | Barriered_NoFlowMods : forall swId lst ep ctrlm ctrlEp,
+    (forall msg, In msg (to_list ctrlm) -> NotFlowMod msg) ->
+    SafeWire swId ctrlEp lst ep ->
+    FlowTableSafe swId (table_at_endpoint ep) ->
+    Barriered swId lst (table_at_endpoint ep) ctrlm
+  | Barriered_OneFlowMod  : forall swId lst ctrlm f tbl ctrlEp,
+    (forall msg, In msg (to_list ctrlm) -> NotFlowMod msg) ->
+    SafeWire swId ctrlEp lst (Endpoint_Barrier (modify_flow_table f tbl)) ->
+    FlowTableSafe swId (modify_flow_table f tbl) ->
+    FlowTableSafe swId tbl ->
+    Barriered swId lst tbl (({|FlowMod f|}) <+> ctrlm).
+
+  Section Barriered.
+
+    Hint Constructors Barriered SafeWire Endpoint.
+
+    Lemma SafeWire_fm_nb_false : forall sw ctrlEp ctrlLst f tbl,
+      SafeWire sw ctrlEp (ctrlLst ++ [FlowMod f]) (Endpoint_FlowMod tbl) ->
+      False.
+    Proof with auto.
+      intros.
+      generalize dependent ctrlEp.
+      induction ctrlLst; intros.
+      + simpl in H. inversion H. subst. inversion H6.
+      + simpl in H.
+        inversion H; subst.
+        - apply IHctrlLst in H5...
+          - apply IHctrlLst in H5...
+          - apply IHctrlLst in H6...
+    Qed.
+
+    Lemma SafeWire_dequeue_PacketOut : forall sw ctrlEp ctrlLst pt pk switchEp,
+      SafeWire sw ctrlEp (ctrlLst ++ [PacketOut pt pk]) switchEp ->
+      SafeWire sw ctrlEp (ctrlLst) switchEp.
+    Proof with auto.
+      intros.
+      generalize dependent ctrlEp.
+      induction ctrlLst; intros.
+      + simpl in H. inversion H. subst...
+      + inversion H; subst...
+    Qed.
+
+
+    Lemma SafeWire_dequeue_BarrierRequest : forall sw ctrlEp ctrlLst xid 
+      switchEp1,
+      SafeWire sw ctrlEp (ctrlLst ++ [BarrierRequest xid]) switchEp1 ->
+      exists switchEp2, SafeWire sw ctrlEp (ctrlLst) switchEp2 /\
+        table_at_endpoint switchEp2 = table_at_endpoint switchEp1.
+    Proof with eauto.
+      intros.
+      generalize dependent ctrlEp.
+      induction ctrlLst; intros.
+      + inversion H; subst.
+        inversion H5. subst.
+        exists (Endpoint_Barrier (table_at_endpoint switchEp1)).
+        split.
+        apply SafeWire_nil.
+        simpl...
+        simpl...
+      + simpl in H.
+        inversion H; subst.
+        * apply IHctrlLst in H5.
+          destruct H5 as [switchEp2 [HSafeWire HEpEq]].
+          exists switchEp2.
+          split; simpl...
+        * apply IHctrlLst in H5.
+          destruct H5 as [switchEp2 [HSafeWire HEpEq]].
+          exists switchEp2.
+          split; simpl...
+        * apply IHctrlLst in H6.
+          destruct H6 as [switchEp2 [HSafeWire HEpEq]].
+          exists switchEp2.
+          split; simpl...
+    Qed.
+
+
+    Lemma SafeWire_dequeue_FlowMod : forall sw ctrlEp ctrlLst f switchEp,
+       SafeWire sw ctrlEp (ctrlLst ++ [FlowMod f]) switchEp ->
+       SafeWire sw ctrlEp ctrlLst (Endpoint_FlowMod (modify_flow_table f (table_at_endpoint switchEp))).
+    Proof with auto.
+      intros.
+      generalize dependent ctrlEp.
+      { induction ctrlLst; intros.
+        + destruct switchEp.
+          simpl in H.
+          inversion H.
+          subst.
+          inversion H6.
+          simpl in H.
+          inversion H.
+          subst.
+          inversion H6.
+          subst.
+          simpl...
+        + simpl in *.
+          inversion H; subst.
+          - apply IHctrlLst in H5...
+          - apply IHctrlLst in H5...
+          - apply IHctrlLst in H6... }
+    Qed.
+
+    Lemma SafeWire_lhs_FlowTableSafe : forall swId lst ep0 ep1,
+      SafeWire swId ep0 lst ep1 ->
+      FlowTableSafe swId (table_at_endpoint ep0).
+    Proof with eauto with datatypes.
+      intros.
+      generalize dependent ep0.
+      generalize dependent ep1.
+      induction lst; intros...
+      + inversion H; subst...
+      + inversion H; subst...
+        apply IHlst in H5...
+    Qed.
+    
+    Lemma SafeWire_app : forall swId ep0 ep1 lst lst0,
+      SafeWire swId ep0 (lst ++ lst0) ep1 ->
+      exists ep01 ep11, 
+        SafeWire swId ep0 lst ep01 /\
+        SafeWire swId ep11 lst0 ep1 /\
+        table_at_endpoint ep01 = table_at_endpoint ep11.
+    Proof with eauto with datatypes.
+      intros.
+      generalize dependent ep0.
+      induction lst; intros...
+      + simpl in H...
+        exists ep0.
+        exists ep0...
+        split...
+        apply SafeWire_nil...
+        eapply SafeWire_lhs_FlowTableSafe...
+      + simpl in H.
+        inversion H; subst...
+        - apply IHlst in H5...
+          destruct H5 as [ep01 [ep11 [H5 [H6 H7]]]]...
+          exists ep01...
+        - apply IHlst in H5...
+          destruct H5 as [ep01 [ep11 [H5 [H6 H7]]]]...
+          exists ep01...
+        - apply IHlst in H6...
+          destruct H6 as [ep01 [ep11 [H6 [H7 H8]]]]...
+          exists ep01...
+    Qed.
+
+    Hint Resolve SafeWire_dequeue_PacketOut SafeWire_dequeue_BarrierRequest SafeWire_dequeue_FlowMod.
+
+    Lemma barriered_pop_FlowMod : forall swId f lst tbl ctrlm,
+      (forall msg, In msg (to_list ctrlm) -> NotFlowMod msg) ->
+      Barriered swId (lst ++ [FlowMod f]) tbl ctrlm ->
+      Barriered swId lst tbl (({|FlowMod f|}) <+> ctrlm).
+    Proof with eauto with datatypes.
+    Admitted.
+
+    Lemma barriered_pop_PacketOut : forall swId pt pk lst tbl ctrlm,
+      Barriered swId (lst ++ [PacketOut pt pk]) tbl ctrlm ->
+      Barriered swId lst tbl (({|PacketOut pt pk|}) <+> ctrlm).
+    Proof with eauto with datatypes.
+      intros.
+      inversion H; subst.
+      + eapply Barriered_NoFlowMods...
+        intros.
+        apply Bag.in_union in H3; simpl in H3.
+        destruct H3 as [[H3|H3]|H3]; subst...
+        inversion H3.
+      + rewrite <- Bag.union_assoc.
+        rewrite <- (Bag.union_comm _ ({|FlowMod f|})).
+        rewrite -> Bag.union_assoc.
+        eapply Barriered_OneFlowMod...
+        intros.
+        apply Bag.in_union in H4; simpl in H4.
+        destruct H4 as [[H4|H4]|H4]; subst...
+        inversion H4.
+    Qed.
+
+    Lemma barriered_pop_BarrierRequest : forall swId xid lst tbl ctrlm,
+      Barriered swId (lst ++ [BarrierRequest xid]) tbl ctrlm ->
+      (forall msg, In msg (to_list ctrlm) -> NotFlowMod msg) ->
+      Barriered swId lst tbl (ctrlm).
+    Proof with eauto with datatypes.
+      intros.
+      rename H0 into X.
+      inversion H; subst.
+      + apply SafeWire_app in H1.
+        destruct H1 as [ep01 [ep11 [J [J0 J1]]]]...
+        assert (table_at_endpoint ep01 = table_at_endpoint ep).
+        { inversion J0; subst... inversion H7; subst... }
+        rewrite <- H1.
+        refine (@Barriered_NoFlowMods swId0 lst ep01 (ctrlm0) ctrlEp _ 
+                 J _)...
+        rewrite -> H1...
+      + assert (NotFlowMod (FlowMod f)).
+        apply X.
+        apply Bag.in_union; simpl...
+        inversion H4.
+    Qed.
+    
+    Lemma Barriered_entails_FlowModSafe : forall swId lst tbl ctrlm,
+      Barriered swId lst tbl ctrlm ->
+      FlowModSafe swId tbl ctrlm.
+    Proof with eauto with datatypes.
+      intros.
+      inversion H; subst...
+      + eapply NoFlowModsInBuffer...
+      + eapply OneFlowModsInBuffer...
+    Qed.
+
+  End Barriered.  
 
   Inductive Invariant : bag switch_le ->  list openFlowLink -> controller -> Prop :=
   | MkP : forall sws ofLinks swsts pktOuts,
-      (forall sw swId0 pendingMsgs switchmLst ctrlmLst,
-         In (SwitchState swId0 pendingMsgs) swsts ->
+      (forall sw swId0 switchmLst ctrlmLst,
          In sw (to_list sws) ->
          In (OpenFlowLink swId0 switchmLst ctrlmLst) ofLinks ->
          swId sw = swId0 ->
-         (forall msg, In msg pendingMsgs -> NotPacketOut msg) /\
-         exists ctrlEp switchEp,
-           SwitchEP sw switchEp /\
-           SafeWire swId0 ctrlEp (rev pendingMsgs ++ ctrlmLst) 
-                                  switchEp) ->
+         exists pendingMsgs,
+           In (SwitchState swId0 pendingMsgs) swsts /\
+           (forall msg, In msg pendingMsgs -> NotPacketOut msg) /\
+           Barriered swId0 (rev pendingMsgs ++ ctrlmLst) (tbl sw) (ctrlm sw)) ->
       Invariant sws ofLinks (Atoms.State pktOuts swsts).
 
   Hint Constructors Invariant.
+
+  (* Also need to show that messages can be popped off. *)
+  Lemma P_entails_FlowTablesSafe : forall sws ofLinks ctrl,
+    Invariant sws ofLinks ctrl ->
+    SwitchesHaveOpenFlowLinks sws ofLinks ->
+    FlowTablesSafe sws.
+  Proof with eauto with datatypes.
+    intros.
+    unfold FlowTablesSafe.
+    intros.
+    inversion H; subst.
+    edestruct H0 as [lnk [HIn HIdEq]]...
+    simpl...
+    destruct lnk.
+    simpl in HIdEq. subst...
+    rename of_to0 into swId0.
+    edestruct H2 as [pendingMsgs [J [J0 J1]]]...
+    simpl in *.
+    eapply Barriered_entails_FlowModSafe...
+  Qed.
+
 
   Lemma controller_recv_pres_P : forall sws ofLinks0 ofLinks1
     ctrl0 ctrl1 swId msg switchm ctrlm,
@@ -58,18 +317,18 @@ Module MakeController (NetAndPol : NETWORK_AND_POLICY) <: ATOMS_AND_CONTROLLER.
     intros.
     inversion H; subst.
     + inversion H0; subst.
-      eapply MkP.
+      eapply MkP...
       intros.
-      apply in_app_iff in H4. simpl in H4.
-      destruct H4 as [H4 | [H4 | H4]]...
-      inversion H4; subst; clear H4.
-      edestruct H1 as [ctrlEp [switchEp [tbl Hsafewire]]]...
+      apply in_app_iff in H3. simpl in H3.
+      destruct H3 as [H3 | [H3 | H3]]...
+      inversion H3; subst; clear H3.
+      edestruct H1 as [msgs [HInSw [HNotPktOuts HBarriered]]]...
     + inversion H0; subst.
       eapply MkP...
       intros.
-      eapply in_app_iff in H3; simpl in H3.
-      destruct H3 as [H3 | [H3 | H3]]...
-      inversion H3; subst; clear H3...
+      eapply in_app_iff in H2; simpl in H2.
+      destruct H2 as [H2 | [H2 | H2]]...
+      inversion H2; subst; clear H2...
   Qed.
 
   Lemma controller_send_pres_P : forall sws ofLinks0 ofLinks1
@@ -87,51 +346,54 @@ Module MakeController (NetAndPol : NETWORK_AND_POLICY) <: ATOMS_AND_CONTROLLER.
     + inversion H0; subst.
       eapply MkP.
       intros.
-      apply in_app_iff in H3; simpl in H3.
-      destruct H3 as [H3 | [H3 | H3]]...
-      inversion H3; subst.
-      edestruct H4 as [HNotPktOuts [ctrlEp [switchEp [tbl Hsafewire]]]]...
+      apply in_app_iff in H2; simpl in H2.
+      destruct H2 as [H2 | [H2 | H2]]...
+      inversion H2; subst.
+      edestruct H4 as [pendingMsgs [HIn [HNotPktOuts HBarriered]]]...
+      exists pendingMsgs.
       split...
-      exists ctrlEp.
-      exists switchEp.
       split...
-      idtac "TODO(arjun): need a lemma that you can always remove a PacketOut and 
-             preserve Safewire with dependencies intact.".
+      (* sticking a PacketOut in the middle is safe *)
       admit.
     + inversion H0; subst.
       eapply MkP.
       intros.
-      destruct sw.
-      simpl in *; subst.
-      destruct (TotalOrder.eqdec swId1 swId0)...
-      - subst.
-        assert (OpenFlowLink swId0 switchmLst ctrlmLst = 
-                OpenFlowLink swId0 switchm0 (msg::ctrlm0)) as X.
-        { idtac "TODO(arjun): need to know that all OF link ids are unique".
-          admit. } 
-        inversion X; clear H3; subst; clear X.
-        assert (SwitchState swId0 pendingMsgs = SwitchState swId0 msgs) as X.
-        { idtac "TODO(arjun): need to know that all state ids are unique".
-          admit. }
-        inversion X; clear H1; subst; clear X.
-        edestruct H4 with 
-          (sw := Switch swId0 pts0 tbl0 inp0 outp0 ctrlm1 switchm1) 
-          (swId1 := swId0)
-          as [HNotPktOuts [ctrlEp [switchEp [tbl Hsafewire]]]]...
+      destruct (eqdec swId1 swId0)...
+      - destruct sw; simpl in *; subst...
+        assert (OpenFlowLink swId0 switchmLst ctrlmLst  = OpenFlowLink swId0 switchm0 (msg::ctrlm0)).
+        { admit. (* all diff *) }
+        inversion H3; subst; clear H3.
+        edestruct H4 as [pendingMsgs [HIn [HNotPktOuts HBarriered]]]...
+        assert (pendingMsgs = msg :: msgs) as X.
+        { admit. (* all diff *) }
+        inversion X; subst.
+        simpl in *.
+        exists msgs...
         split...
-        assert (msg::msgs = [msg] ++ msgs) as X...
-        rewrite -> X in Hsafewire; clear X.
-        rewrite -> rev_app_distr in Hsafewire.
-        rewrite <- app_assoc in Hsafewire.
-        simpl in Hsafewire...
-      - edestruct H4 with (sw := Switch swId1 pts0 tbl0 inp0 outp0 ctrlm1 switchm1) 
-                            (swId1:=swId1) as [ctrlEp [switchEp [tbl Hsafewire]]]...
-        { apply in_app_iff in H1; simpl in H1.
-          destruct H1 as [H1 | [H1 | H1]]...
-          inversion H1; subst. contradiction n... }
-        { apply in_app_iff in H3; simpl in H3.
-          destruct H3 as [H3 | [H3 | H3]]...
-          inversion H3; subst. contradiction n... }
+        split...
+        rewrite <- app_assoc in HBarriered.
+        simpl in HBarriered...
+      - destruct sw; subst; simpl in *.
+        apply in_app_iff in H2; simpl in H2.
+        { destruct H2 as [H2|[H2|H2]].
+          + edestruct H4 with (swId1 := swId2) as [pendingMsgs [HIn [HNotPktOuts HBarriered]]]...
+            simpl in *.
+            exists pendingMsgs...
+            split...
+            apply in_app_iff in HIn; simpl in HIn.
+            destruct HIn as [HIn|[HIn|HIn]]...
+            inversion HIn; subst.
+            contradiction n...
+          + inversion H2; subst.
+            contradiction n...
+          + edestruct H4 with (swId1 := swId2) as [pendingMsgs [HIn [HNotPktOuts HBarriered]]]...
+            simpl in *.
+            exists pendingMsgs...
+            split...
+            apply in_app_iff in HIn; simpl in HIn.
+            destruct HIn as [HIn|[HIn|HIn]]...
+            inversion HIn; subst.
+            contradiction n... }
   Qed.
 
   Lemma controller_step_pres_P : forall sws ofLinks ctrl0 ctrl1,
@@ -146,63 +408,6 @@ Module MakeController (NetAndPol : NETWORK_AND_POLICY) <: ATOMS_AND_CONTROLLER.
   Local Open Scope bag_scope.
   Hint Constructors NotFlowMod.
 
-  Lemma SwitchEP_vary : forall swId0 pts0 tbl0 inp0 outp0 cms0 sms0 ep
-                               inp1 outp1 sms1,
-    SwitchEP (Switch swId0 pts0 tbl0 inp0 outp0 cms0 sms0) ep ->
-    SwitchEP (Switch swId0 pts0 tbl0 inp1 outp1 cms0 sms1) ep.
-  Proof with auto with datatypes.
-    intros.
-    inversion H; subst...
-    + eapply NoFlowModsInBuffer...
-    + eapply OneFlowModInBuffer...
-      intros.
-      apply H8...
-  Qed.
-
-  Lemma SwitchEP_packetOut : forall swId0 pts0 tbl0 inp0 outp0 cms0 sms0 ep
-                               pt pk,
-    SwitchEP (Switch swId0 pts0 tbl0 inp0 outp0 (({|PacketOut pt pk|}) <+> cms0) sms0) ep <->
-    SwitchEP (Switch swId0 pts0 tbl0 inp0 outp0 cms0 sms0) ep.
-  Proof with auto with datatypes.
-    split.
-    { intros.
-    inversion H; subst...
-    + eapply NoFlowModsInBuffer...
-      intros.
-      apply H8.
-      apply Bag.in_union...
-    + assert (In (PacketOut pt pk) (to_list (({|FlowMod f|}) <+> ctrlm1))).
-      { rewrite <- H9. apply Bag.in_union; simpl... }
-      apply Bag.in_union in H0. simpl in H0.
-      destruct H0 as [[H0 | H0] | H0]; try solve[inversion H0].
-      destruct (Bag.in_split TotalOrder_fromController _ _ H0) as [rest Heq].
-      subst.
-      rewrite <- Bag.union_assoc in H9.
-      rewrite -> (Bag.union_comm _ ({|FlowMod f|})) in H9.
-      rewrite -> Bag.union_assoc in H9.
-      apply Bag.pop_union_l in H9.
-      subst.
-      eapply OneFlowModInBuffer...
-      intros.
-      apply H8.
-      apply Bag.in_union... }
-    intros.
-    inversion H; subst...
-    + apply NoFlowModsInBuffer...
-      intros.
-      apply Bag.in_union in H0; simpl in H0.
-      destruct H0 as [[H0|H0]|H0]...
-      subst...
-      inversion H0.
-    + rewrite <- Bag.union_assoc.
-      rewrite <-(Bag.union_comm _ ({|FlowMod f|})).
-      rewrite -> Bag.union_assoc.
-      apply OneFlowModInBuffer with (ctrlm0 := (({|PacketOut pt pk|}) <+> ctrlm1))... 
-      intros.
-      apply Bag.in_union in H0; simpl in H0.
-      destruct H0 as [[H0|H0]|H0]...
-      subst... inversion H0.
-  Qed.
 
   Lemma Invariant_ofLink_vary : forall sws swId switchm0 switchm1 ctrlm 
                                    ofLinks0 ofLinks1 ctrl,
@@ -217,10 +422,11 @@ Module MakeController (NetAndPol : NETWORK_AND_POLICY) <: ATOMS_AND_CONTROLLER.
     inversion H; subst.
     eapply MkP.
     intros.
-    apply in_app_iff in H3; simpl in H3.
-    destruct H3 as [H3 | [H3 | H3]]...
+    apply in_app_iff in H2; simpl in H2.
+    destruct H2 as [H2 | [H2 | H2]]...
     destruct sw. simpl in *. subst.
-    inversion H3; clear H3; subst...
+    inversion H2; clear H2; subst...
+    edestruct H0 as [pendingMsgs0 [HIn [HNotPktOuts HBarriered]]]...
   Qed.
 
   Lemma Invariant_sw_vary : forall swId pts tbl inp outp cms sms sws
@@ -236,39 +442,26 @@ Module MakeController (NetAndPol : NETWORK_AND_POLICY) <: ATOMS_AND_CONTROLLER.
     inversion H; subst.
     eapply MkP.
     intros.
-    apply Bag.in_union in H2; simpl in H2.
-    destruct H2 as [[H2 | H2] | H2]...
+    apply Bag.in_union in H1; simpl in H1.
+    destruct H1 as [[H1 | H1] | H1]...
     - subst. simpl in *.
       remember (Switch swId0 pts0 tbl0 inp0 outp0 cms sms) as sw.
       assert (swId0 = swId sw) as X.
       { subst. simpl... }
-      edestruct H0 as [HNotPktOuts [ctrlEp [switchEp [Hep Hsafewire]]]]...
+      edestruct H0 as [msgs [HIn [HNotPktOuts HBarriered]]]...
       { apply Bag.in_union. left. simpl... }
+      exists msgs...
       split...
-      exists ctrlEp.
-      exists switchEp.
       split...
-      eapply SwitchEP_vary... rewrite -> Heqsw in Hep. exact Hep.
-    - inversion H2.
-    - destruct sw. simpl in *.
-      rewrite -> H4 in *; clear swId2 H4.
-      assert (swId1 = swId (Switch swId1 pts1 tbl1 inp1 outp1 ctrlm0 switchm0)) as X.
-      { simpl... }
-      edestruct H0 as [HNotPktOuts [ctrlEp [switchEp [Hep Hsafewire]]]]...
+      destruct sw; subst; simpl in *.
+      inversion Heqsw; subst...
+    - inversion H1.
+    - destruct sw. simpl in *; subst.
+      edestruct H0 as [msgs [HIn [HNotPktOuts HBarriered]]]...
       { apply Bag.in_union. right... }
+      simpl...
+      exists msgs...
   Qed.
-  
-  Lemma SafeWire_switchEp_safe : forall swId ctrlEp lst switchEp,
-    SafeWire swId ctrlEp lst switchEp ->
-    FlowTableSafe swId (table_at_endpoint switchEp).
-  Proof with eauto with datatypes.
-    intros.
-    generalize dependent ctrlEp.
-    induction lst; intros.
-    inversion H; subst...
-    inversion H; subst...
-  Qed.
-
 
   Lemma step_preserves_P : forall sws0 sws1 links0 links1 ofLinks0 ofLinks1 
     ctrl0 ctrl1 obs,
@@ -281,201 +474,129 @@ Module MakeController (NetAndPol : NETWORK_AND_POLICY) <: ATOMS_AND_CONTROLLER.
     intros.
     destruct ctrl1.
     inversion H0; subst.
+    rename H0 into HInvariant.
     inversion H; subst.
-    - eapply Invariant_sw_vary...
-    - eapply MkP.
+    + eapply Invariant_sw_vary...
+    + eapply MkP.
       intros.
-      apply Bag.in_union in H3; simpl in H3.
-      destruct H3 as [[H3 | H3] | H3]...
-      + subst. simpl in *.
-        remember (Switch swId0 pts0 tbl0 inp0 outp0 (({|Atoms.FlowMod fm|}) <+> ctrlm0) switchm0) as swInit.
-        destruct H1 with 
-          (sw := swInit)
-          (pendingMsgs:=pendingMsgs)
-          (swId0:=swId0)
-          (switchmLst:=switchmLst)
-          (ctrlmLst:=ctrlmLst) as [HNotPktOuts [ctrlEp [swEp [Hep Hsafewire]]]]...
-        { apply Bag.in_union. simpl... }
-        { rewrite -> HeqswInit... }
-        split...
-        exists ctrlEp.
-        { inversion Hep; subst.
-          + inversion H6; subst.
-            assert (NotFlowMod (FlowMod fm)) as Hcontra.
-            { apply H3. apply Bag.in_union. simpl... }
-            inversion Hcontra.
-          + inversion H7; subst; clear H7.
-            assert (({|FlowMod f|}) <+> ctrlm2 = ({|FlowMod fm|}) <+> ctrlm0) as Heq.
-            { apply Bag.ordered_irr. unfold to_list. simpl. exact H13.  }
-            clear H13.
-            assert (In (FlowMod f) (to_list (({|FlowMod fm|}) <+> ctrlm0))) as X.
-            { 
-              rewrite <- Heq.
-              apply Bag.in_union. simpl... }
-            apply Bag.in_union in X; simpl in X.
-            destruct X as [[X | X] | X].
-            inversion X; subst; clear X.
-            assert (ctrlm2 = ctrlm0) as X.
-            { rewrite -> Bag.pop_union_l. exact Heq. }
-            subst; clear Heq.
-            eexists.
-            split...
-            eapply NoFlowModsInBuffer...
-            inversion X.
-            assert (In (FlowMod fm) (to_list (({|FlowMod f|}) <+> ctrlm2))) as Y.
-            { rewrite -> Heq. apply Bag.in_union; simpl... }
-            apply Bag.in_union in Y; simpl in Y.
-            destruct Y as [[Y | Y] | Y].
-            inversion Y; subst.
-            rewrite <- Bag.pop_union_l in Heq.
-            subst.
-            assert (NotFlowMod (FlowMod fm)) as Hcontra...
-            inversion Hcontra.
-            inversion Y.
-            apply H3 in Y. inversion Y. }
-      + inversion H3.
-      + edestruct H1...
-        { apply Bag.in_union. right... }
-    - eapply MkP.
-      intros.
-      apply Bag.in_union in H3; simpl in H3.
-      destruct H3 as [[H3 | H3] | H3]...
-      + subst. simpl in *.
-        remember (Switch swId0 pts0 tbl0 inp0 outp0 (({|PacketOut pt pk|}) <+> ctrlm0) switchm0) as swInit.
-        destruct H1 with 
-          (sw := swInit)
-          (pendingMsgs:=pendingMsgs)
-          (swId0:=swId0)
-          (switchmLst:=switchmLst)
-          (ctrlmLst:=ctrlmLst) as [HNotPktOuts [ctrlEp [swEp [Hep Hsafewire]]]]...
-        { apply Bag.in_union. simpl... }
-        { rewrite -> HeqswInit... }
-        split...
-        exists ctrlEp.
-        rewrite -> HeqswInit in Hep.
-        apply SwitchEP_packetOut in Hep.
-        apply SwitchEP_vary with (inp1:=inp0) (outp1:=({|(pt,pk)|}) <+> outp0) (sms1:=switchm0) in Hep.
-        exists swEp.
-        split...
-      + inversion H3.
-      + edestruct H1...
-        { apply Bag.in_union... }
-    - eapply Invariant_sw_vary...
-    - eapply Invariant_sw_vary...
-    - eapply controller_step_pres_P...
-    - eapply controller_recv_pres_P...
-    - eapply controller_send_pres_P...
-    - eapply Invariant_sw_vary...
+      apply Bag.in_union in H0; simpl in H0.
+      destruct H0 as [[H0 | H0] | H0]...
+      - subst; simpl in *.
+        edestruct H1 as [msgs [HIn [HNotPktOuts HBarriered]]]...
+        apply Bag.in_union. simpl. left. left. reflexivity. simpl...
+        simpl in *.
+        inversion HBarriered; subst.
+        * assert (NotFlowMod (FlowMod fm)) as X.
+          apply H0.
+          apply Bag.in_union; simpl...
+          inversion X.
+        * exists msgs...
+          split...
+          split...
+          assert (fm = f).
+          { admit. (* trivial by H0 *) }
+          assert (ctrlm1 = ctrlm0).
+          { admit. (* trivial by H0 *) }
+          subst.
+          assert (table_at_endpoint (Endpoint_Barrier (modify_flow_table f tbl0)) = 
+                  modify_flow_table f tbl0) as J.
+          { simpl... }
+          rewrite <- J.
+          eapply Barriered_NoFlowMods...
+      - inversion H0.
+      - subst; simpl in *.
+        edestruct H1 as [msgs [HIn [HNotPktOuts HBarriered]]]...
+        apply Bag.in_union...
+     + (* processing a packet produces ctrlm messges. *)
+       admit.
+    + eapply Invariant_sw_vary...
+    + eapply Invariant_sw_vary...
+    + eapply controller_step_pres_P...
+    + eapply controller_recv_pres_P...
+    + eapply controller_send_pres_P...
+    + eapply Invariant_sw_vary...
       eapply Invariant_ofLink_vary...
-    - eapply MkP.
+    + eapply MkP.
       intros.
       destruct sw; subst; simpl in *.
       destruct (TotalOrder.eqdec swId0 swId2).
-      + subst.
+      - subst.
         assert (OpenFlowLink swId2 switchmLst ctrlmLst = 
                 OpenFlowLink swId2 fromSwitch0 fromCtrl) as X.
         { idtac "TODO(arjun): need to know that all OF link ids are unique".
           admit. } 
-        inversion X; clear H4; subst; clear X.
+        inversion X; clear H2; subst; clear X.
         assert (Switch swId2 pts1 tbl1 inp1 outp1 ctrlm0 switchm1 =
                 Switch swId2 pts0 tbl0 inp0 outp0 ({||}) (({|BarrierReply xid|})<+>switchm0)) as X.
         { idtac "TODO(arjun): need to know that all switch  ids are unique".
           admit. } 
-        inversion X; clear H3; subst; clear X.
-        edestruct H1 as [HPktOuts [ctrlEp [switchEp [J J0]]]]...
+        inversion X; clear H0; subst; clear X.
+        edestruct H1 as [msgs [HIn [HNotPktOuts HBarriered]]]...
         { apply Bag.in_union. left. simpl. left. reflexivity. }
         { simpl... }
+        simpl in *.
+        exists msgs...
         split...
-        rewrite -> app_assoc in J0.
-        remember (rev pendingMsgs ++ fromCtrl) as lst.
-        destruct lst.
-        * simpl in J0.
-          inversion J0; subst.
-          inversion H8; subst.
-          apply SwitchEP_vary with (inp1:=inp0) (outp1:=outp0) (sms1:=({|BarrierReply xid|})<+>switchm0) in J.
-          exists switchEp.
-          exists switchEp.
-          split...
-        * apply SwitchEP_vary with (inp1:=inp0) (outp1:=outp0) (sms1:=({|BarrierReply xid|})<+>switchm0) in J.
-          apply SafeWire_dequeue_BarrierRequest in J0.
-          destruct J0 as [switchEp' [Hsafewire Htbl]].
-          exists ctrlEp, switchEp'.
-          split...
-          apply NoFlowModsInBuffer...
-          intros. simpl in H3. inversion H3.
-          inversion J; subst...
-          idtac "TODO(arjun): stupid contradiction in H12 that is easy to discharge.".
-          admit. 
-      + assert (In (Switch swId2 pts1 tbl1 inp1 outp1 ctrlm0 switchm1) (to_list sws)) as J.
-        { apply Bag.in_union in H3; simpl in H3.
-          destruct H3 as [[H3 | H3] | H3]...
-          inversion H3; subst. contradiction n...
-          inversion H3. }
-        clear H3.
-        eapply H1...
-        { apply Bag.in_union... }
-        { instantiate (1:=switchmLst).
-          assert (In (OpenFlowLink swId2 switchmLst ctrlmLst) (ofLinks2 ++ ofLinks3)).
-          { apply in_app_iff in H4; simpl in H4. 
-            destruct H4 as [H4 | [H4 | H4]]...
-            inversion H4; subst; contradiction n... }
-          apply in_app_iff in H3.
-          destruct H3... }
-    - eapply MkP.
+        split...
+        eapply barriered_pop_BarrierRequest...
+        rewrite -> app_assoc in HBarriered...
+        intros.
+        simpl in H0.
+        inversion H0.
+      - apply Bag.in_union in H0; simpl in H0.
+        destruct H0 as [[H0|H0]|H0].
+        * inversion H0; subst. contradiction n...
+        * inversion H0.
+        * edestruct H1 with (swId1:=swId2) as [msgs [HIn [HNotPktOuts HBarriered]]]...
+          apply Bag.in_union...
+          apply in_app_iff in H2; simpl in H2.
+          destruct H2 as [H2|[H2|H2]]...
+          inversion H2; subst; contradiction n...
+          simpl...
+          exists msgs...
+    + eapply MkP.
       intros.
       destruct sw; subst; simpl in *.
       destruct (TotalOrder.eqdec swId0 swId2).
-      + subst.
+      - subst.
         assert (OpenFlowLink swId2 switchmLst ctrlmLst = 
                 OpenFlowLink swId2 fromSwitch0 fromCtrl) as X.
         { idtac "TODO(arjun): need to know that all OF link ids are unique".
           admit. } 
-        inversion X; clear H4; subst; clear X.
+        inversion X; clear H2; subst; clear X.
         assert (Switch swId2 pts1 tbl1 inp1 outp1 ctrlm1 switchm1 =
-                Switch swId2 pts0 tbl0 inp0 outp0 (({|msg|}) <+> ctrlm0) switchm0) as X.
+                Switch swId2 pts0 tbl0 inp0 outp0 ({|msg|} <+> ctrlm0) switchm0) as X.
         { idtac "TODO(arjun): need to know that all switch  ids are unique".
           admit. } 
-        inversion X; clear H3; subst; clear X.
-        edestruct H1 as [HPktOuts [ctrlEp [switchEp [J J0]]]]...
+        inversion X; clear H0; subst; clear X.
+        edestruct H1 as [msgs [HIn [HNotPktOuts HBarriered]]]...
         { apply Bag.in_union. left. simpl. left. reflexivity. }
         { simpl... }
+        simpl in *.
+        exists msgs...
         split...
-        rewrite -> app_assoc in J0.
-        { destruct msg.
-          + apply SafeWire_dequeue_PacketOut in J0.
-            exists ctrlEp, switchEp.
-            split...
-            apply SwitchEP_packetOut...
-          + idtac "TODO(arjun): barriers on bags again ffs".
-            admit.
-          + remember J0 as J1 eqn:Z; clear Z.
-            apply SafeWire_dequeue_FlowMod in J0.
-            exists ctrlEp, (Endpoint_NoBarrier (modify_flow_table f (table_at_endpoint switchEp))).
-            split...
-            { inversion J; subst.
-              + simpl in *.
-                destruct switchEp.
-                simpl in *.
-                apply SafeWire_fm_nb_false in J1. inversion J1. 
-                eapply OneFlowModInBuffer...
-                simpl in *.
-                apply SafeWire_switchEp_safe in J0...
-              + apply SafeWire_fm_nb_false in J1. inversion J1.  } }
-      + assert (In (Switch swId2 pts1 tbl1 inp1 outp1 ctrlm1 switchm1) (to_list sws)) as J.
-        { apply Bag.in_union in H3; simpl in H3.
-          destruct H3 as [[H3 | H3] | H3]...
-          inversion H3; subst. contradiction n...
-          inversion H3. }
-        clear H3.
-        eapply H1...
-        { apply Bag.in_union... }
-        { instantiate (1:=switchmLst).
-          assert (In (OpenFlowLink swId2 switchmLst ctrlmLst) (ofLinks2 ++ ofLinks3)).
-          { apply in_app_iff in H4; simpl in H4. 
-            destruct H4 as [H4 | [H4 | H4]]...
-            inversion H4; subst; contradiction n... }
-          apply in_app_iff in H3.
-          destruct H3... }
+        split...
+        destruct msg.
+        * eapply barriered_pop_PacketOut...
+          rewrite -> app_assoc in HBarriered...
+        * inversion H6.
+        * { inversion HBarriered; subst.
+            + eapply barriered_pop_FlowMod...
+              rewrite <- app_assoc...
+            + clear H HInvariant H1.  move H2 after HBarriered.
+              admit. }
+      - intros.
+        apply Bag.in_union in H0; simpl in H0.
+        destruct H0 as [[H0|H0]|H0].
+        * inversion H0; subst. contradiction n...
+        * inversion H0.
+        * edestruct H1 with (swId1:=swId2) as [msgs [HIn [HNotPktOuts HBarriered]]]...
+          apply Bag.in_union...
+          apply in_app_iff in H2; simpl in H2.
+          destruct H2 as [H2|[H2|H2]]...
+          inversion H2; subst; contradiction n...
+          simpl...
+          exists msgs...
   Qed.
 
   Definition relate_helper (sd : srcDst) : swPtPks :=
@@ -615,50 +736,8 @@ Module MakeController (NetAndPol : NETWORK_AND_POLICY) <: ATOMS_AND_CONTROLLER.
        exists (lps : swPtPks),
          (select_packet_in sw m) <+> lps = relate_controller ctrl1.
 
-  Lemma SafeWire_app : forall swId ep0 ep1 lst lst0,
-    SafeWire swId ep0 (lst ++ lst0) ep1 ->
-    exists ep, SafeWire swId ep lst0 ep1.
-  Proof with eauto with datatypes.
-    intros.
-    generalize dependent ep0.
-    induction lst; intros...
-    simpl in H.
-    inversion H; subst...
-  Qed.
-
-
-  Lemma SwitchEP_injective : forall sw ep0 ep1,
-    SwitchEP sw ep0 ->
-    SwitchEP sw ep1 ->
-    table_at_endpoint ep0 = table_at_endpoint ep1.
-  Proof with eauto with datatypes.
-    intros.
-    destruct sw.
-    inversion H; inversion H0; subst...
-    + assert (NotFlowMod (FlowMod f)).
-      apply H9.
-      apply Bag.in_union; simpl...
-      inversion H1.
-    + assert (NotFlowMod (FlowMod f)) as X; subst...
-      apply H20.
-      apply Bag.in_union; simpl...
-      inversion X.
-    + assert (f = f0) as X.
-      { assert (In (FlowMod f) (to_list (({|FlowMod f0|}) <+> ctrlm4))) as X.
-        rewrite <- H21.
-        apply Bag.in_union; simpl...
-        apply Bag.in_union in X.
-        simpl in X; destruct X as [[X|X]|X].
-        inversion X...
-        inversion X.
-        assert (NotFlowMod (FlowMod f)) as Y.
-        apply H20...
-        inversion Y. }
-      subst...
-  Qed.
-
   Lemma SafeWire_injective_lhs : forall swId ep0 ep1 lst tbl,
-    SafeWire swId ep0 lst (Endpoint_NoBarrier tbl) ->
+    SafeWire swId ep0 lst (Endpoint_FlowMod tbl) ->
     SafeWire swId ep1 lst (Endpoint_Barrier tbl) ->
     table_at_endpoint ep0 = table_at_endpoint ep1.
   Proof with eauto with datatypes.
@@ -680,7 +759,7 @@ Module MakeController (NetAndPol : NETWORK_AND_POLICY) <: ATOMS_AND_CONTROLLER.
 
   Lemma SafeWire_insane_1 : forall swId ctrlEp0 lst tbl tbl0,
     SafeWire swId ctrlEp0 lst (Endpoint_Barrier tbl) ->
-    SafeWire swId (Endpoint_Barrier tbl0) lst (Endpoint_NoBarrier tbl) ->
+    SafeWire swId (Endpoint_Barrier tbl0) lst (Endpoint_FlowMod tbl) ->
     SafeWire swId (Endpoint_Barrier tbl0) lst (Endpoint_Barrier tbl).
   Proof with eauto with datatypes.
     intros.
@@ -701,95 +780,5 @@ Module MakeController (NetAndPol : NETWORK_AND_POLICY) <: ATOMS_AND_CONTROLLER.
         exact H.
       - inversion H0.
   Qed.
-
-  Lemma SafeWire_insane_2 : forall swId ctrlEp0 lst tbl tbl0,
-    SafeWire swId ctrlEp0 lst (Endpoint_NoBarrier tbl) ->
-    SafeWire swId (Endpoint_Barrier tbl0) lst (Endpoint_Barrier tbl) ->
-    SafeWire swId (Endpoint_Barrier tbl0) lst (Endpoint_NoBarrier tbl).
-  Proof with eauto with datatypes.
-    intros.
-    generalize dependent ctrlEp0.
-    induction lst; intros...
-    + admit. (* need to relax SafeWire_nil. *)
-    + destruct a.
-      - eapply SafeWire_PktOut. 
-        inversion H0; subst.
-        eapply IHlst...
-        inversion H...
-      - assert (table_at_endpoint ctrlEp0 =  table_at_endpoint (Endpoint_Barrier tbl1)) as X.
-        { eapply SafeWire_injective_lhs... }
-        destruct ctrlEp0. 
-        inversion H.
-        simpl in X.
-        subst.
-        exact H.
-      - inversion H0.
-  Qed.
-
-  Lemma ControllerFMS : forall swId ctrl0 ctrl1 msg ctrlm
-    switchm sws links ofLinks0 ofLinks1 switchEp ctrlEp0
-    pts tbl inp outp swCtrlm swSwitchm,
-    SafeWire swId ctrlEp0 ctrlm switchEp ->
-    P sws
-      (ofLinks0 ++ (OpenFlowLink swId switchm ctrlm) :: ofLinks1)
-      ctrl0 ->
-    controller_send ctrl0 ctrl1 swId msg ->
-    step
-      (State
-        sws
-        links
-        (ofLinks0 ++ (OpenFlowLink swId switchm ctrlm) :: ofLinks1)
-        ctrl0)
-      None
-      (State
-         sws
-         links
-         (ofLinks0 ++ (OpenFlowLink swId switchm (msg :: ctrlm)) :: ofLinks1)
-         ctrl1) ->
-     In (Switch swId pts tbl inp outp swCtrlm swSwitchm) (to_list sws) ->
-     SwitchEP (Switch swId pts tbl inp outp swCtrlm swSwitchm) switchEp ->
-      exists ctrlEp1,
-        SafeWire swId ctrlEp1 (msg :: ctrlm) switchEp.
-    Proof with eauto with datatypes.
-      intros.
-      inversion H1; subst.
-      + exists ctrlEp0.
-        apply SafeWire_PktOut...
-      + remember H2 as J eqn:X; clear X.
-        apply step_preserves_P in H2...
-        clear H1.
-        inversion H2; subst.
-        edestruct H7 as [HNotPktOuts [ctrlEp2 [switchEp0 [Hep Hsafewire]]]]...
-        destruct msg.
-        - exists ctrlEp0.
-          apply SafeWire_PktOut...
-        - exists (Endpoint_Barrier (table_at_endpoint ctrlEp0)).
-          apply SafeWire_BarrierRequest...
-        - assert (table_at_endpoint switchEp = table_at_endpoint switchEp0) as X.
-          { eapply SwitchEP_injective... }
-          destruct switchEp, switchEp0; simpl in X; subst.
-          * apply SafeWire_app in Hsafewire.
-            destruct Hsafewire as [ctrlEp3 Hsafewire].
-            inversion Hsafewire; subst.
-            exists (Endpoint_NoBarrier (modify_flow_table f tbl1)).
-            eapply SafeWire_FlowMod...
-          * apply SafeWire_app in Hsafewire.
-            destruct Hsafewire as [ctrlEp3 Hsafewire].
-            inversion Hsafewire; subst.
-            exists (Endpoint_NoBarrier (modify_flow_table f tbl1)).
-            eapply SafeWire_FlowMod...
-            eapply SafeWire_insane_2...
-          * apply SafeWire_app in Hsafewire.
-            destruct Hsafewire as [ctrlEp3 Hsafewire].
-            inversion Hsafewire; subst.
-            exists (Endpoint_NoBarrier (modify_flow_table f tbl1)).
-            eapply SafeWire_FlowMod...
-            eapply SafeWire_insane_1...
-          * apply SafeWire_app in Hsafewire.
-            destruct Hsafewire as [ctrlEp3 Hsafewire].
-            inversion Hsafewire; subst.
-            exists (Endpoint_NoBarrier (modify_flow_table f tbl1)).
-            eapply SafeWire_FlowMod...
-    Qed.
 
 End MakeController.
