coq/FwOF/FwOFWellFormedness.v
@@ -6,717 +6,32 @@ Require Import Common.Bisimulation.
 Require Import Common.AllDiff.
 Require Import Bag.Bag2.
 Require Import FwOF.FwOFSignatures.
+Require FwOF.FwOFWellFormednessLemmas.
 
 Local Open Scope list_scope.
 Local Open Scope bag_scope.
 
-Module Make (AtomsAndController_ : ATOMS_AND_CONTROLLER) <: RELATION.
+Module Make (Import RelationDefinitions : RELATION_DEFINITIONS) <: RELATION.
 
-  Module AtomsAndController := AtomsAndController_.
-  Import AtomsAndController_.
+  Module RelationDefinitions := RelationDefinitions.
+  Import AtomsAndController.
   Import Machine.
   Import Atoms.
-
-  Definition affixSwitch (sw : switchId) (ptpk : portId * packet) :=
-    match ptpk with
-      | (pt,pk) => (sw,pt,pk)
-    end.
-
-  Definition FlowTablesSafe (sws : bag switch_le) : Prop :=
-    forall swId pts tbl inp outp ctrlm switchm,
-      In (Switch swId pts tbl inp outp ctrlm switchm) (to_list sws) ->
-      FlowTableSafe swId tbl.
-
-  Definition ConsistentDataLinks (links : list dataLink) : Prop :=
-    forall (lnk : dataLink),
-      In lnk links ->
-      topo (src lnk) = Some (dst lnk).
-
-  Definition LinkHasSrc (sws : bag switch_le) (link : dataLink) : Prop :=
-    exists switch,
-      In switch (to_list sws) /\
-      fst (src link) = swId switch /\
-      In (snd (src link)) (pts switch).
-
-  Definition LinkHasDst (sws : bag switch_le) (link : dataLink) : Prop :=
-    exists switch,
-      In switch (to_list sws) /\
-      fst (dst link) = swId switch /\
-      In (snd (dst link)) (pts switch).
-
-  Definition LinksHaveSrc (sws : bag switch_le) (links : list dataLink) :=
-    forall link, In link links -> LinkHasSrc sws link.
-
-  Definition LinksHaveDst (sws : bag switch_le) (links : list dataLink) :=
-    forall link, In link links -> LinkHasDst sws link.
-
-  Definition UniqSwIds (sws : bag switch_le) := AllDiff swId (to_list sws).
-
-  Definition ofLinkHasSw (sws : bag switch_le) (ofLink : openFlowLink) :=
-    exists sw,
-      In sw (to_list sws) /\
-      of_to ofLink = swId sw.
-
-  Definition OFLinksHaveSw (sws : bag switch_le) (ofLinks : list openFlowLink) :=
-    forall ofLink, In ofLink ofLinks -> ofLinkHasSw sws ofLink.
-
-  Definition DevicesFromTopo (devs : state) :=
-    forall swId0 swId1 pt0 pt1,
-      Some (swId0,pt0) = topo (swId1,pt1) ->
-      exists sw0 sw1 lnk,
-        In sw0 (to_list (switches devs)) /\
-        In sw1 (to_list (switches devs)) /\
-        In lnk (links devs) /\
-        swId sw0 = swId0 /\
-        swId sw1 = swId1 /\
-        src lnk = (swId1,pt1) /\
-        dst lnk = (swId0, pt0).
-
-  Definition SwitchesHaveOpenFlowLinks (devs : state) :=
-    forall sw,
-      In sw (to_list (switches devs)) ->
-      exists ofLink,
-        In ofLink (ofLinks devs) /\
-        swId sw = of_to ofLink.
-
-  Record concreteState := ConcreteState {
-    devices : state;
-    concreteState_flowTableSafety : FlowTablesSafe (switches devices);
-    concreteState_consistentDataLinks : ConsistentDataLinks (links devices);
-    linksHaveSrc : LinksHaveSrc (switches devices) (links devices);
-    linksHaveDst : LinksHaveDst (switches devices) (links devices);
-    uniqSwIds : UniqSwIds (switches devices);
-    allFMS : AllFMS (switches devices) (ofLinks devices);
-    ctrlP : P (switches devices) (ofLinks devices) (ctrl devices);
-    uniqOfLinkIds : AllDiff of_to (ofLinks devices);
-    ofLinksHaveSw : OFLinksHaveSw (switches devices) (ofLinks devices);
-    devicesFromTopo : DevicesFromTopo devices;
-    swsHaveOFLinks : SwitchesHaveOpenFlowLinks devices
-  }.
-
-  Implicit Arguments ConcreteState [].
-
-  Definition concreteStep (st : concreteState) (obs : option observation)
-    (st0 : concreteState) :=
-    step (devices st) obs (devices st0).
-
-  Inductive abstractStep : abst_state -> option observation -> abst_state -> 
-    Prop := 
-  | AbstractStep : forall sw pt pk lps,
-    abstractStep
-      ({| (sw,pt,pk) |} <+> lps)
-      (Some (sw,pt,pk))
-      (unions (map (transfer sw) (abst_func sw pt pk)) <+> lps).
-
-  Definition relate_switch (sw : switch) : abst_state :=
-    match sw with
-      | Switch swId _ tbl inp outp ctrlm switchm =>
-        from_list (map (affixSwitch swId) (to_list inp)) <+>
-        unions (map (transfer swId) (to_list outp)) <+>
-        unions (map (select_packet_out swId) (to_list ctrlm)) <+>
-        unions (map (select_packet_in swId) (to_list switchm))
-    end.
-
-  Definition relate_dataLink (link : dataLink) : abst_state :=
-    match link with
-      | DataLink _ pks (sw,pt) =>
-        from_list (map (fun pk => (sw,pt,pk)) pks)
-    end.
-
-  Definition relate_openFlowLink (link : openFlowLink) : abst_state :=
-    match link with
-      | OpenFlowLink sw switchm ctrlm =>
-        unions (map (select_packet_out sw) ctrlm) <+>
-        unions (map (select_packet_in sw) switchm)
-    end.
-
-  Definition relate (st : state) : abst_state :=
-    unions (map relate_switch (to_list (switches st))) <+>
-    unions (map relate_dataLink (links st)) <+>
-    unions (map relate_openFlowLink (ofLinks st)) <+>
-    relate_controller (ctrl st).
-
-  Definition bisim_relation : relation concreteState abst_state :=
-    fun (st : concreteState) (ast : abst_state) => 
-      ast = (relate (devices st)).
-
-  Lemma LinksHaveSrc_untouched : forall 
-    {swId tbl pts sws links
-    inp outp ctrlm switchm tbl' inp' outp' ctrlm' switchm' },
-    LinksHaveSrc 
-      ({| Switch swId pts tbl inp outp ctrlm switchm |} <+> sws)  links ->
-    LinksHaveSrc 
-      ({| Switch swId pts tbl' inp' outp' ctrlm' switchm' |} <+> sws)
-      links.
-  Proof with auto.
-    intros.
-    unfold LinksHaveSrc in *.
-    intros.
-    apply H in H0. clear H.
-    unfold LinkHasSrc in *.
-    destruct H0 as [sw [HMem [HEq HIn]]].
-    simpl in HMem.
-    rewrite -> Bag.in_union in HMem.
-    destruct HMem.
-    + destruct sw.
-      simpl in *.
-      destruct H.
-      inversion H.
-      subst.
-      eexists.
-      split. 
-      apply Bag.in_union. left. simpl. left. reflexivity.
-      simpl...
-      inversion H.
-    + exists sw.
-      split...
-      simpl...
-      apply Bag.in_union...
-  Qed.
-
-  Lemma LinksHaveDst_untouched : forall 
-    {swId tbl pts sws links
-    inp outp ctrlm switchm tbl' inp' outp' ctrlm' switchm' },
-    LinksHaveDst
-      ({| Switch swId pts tbl inp outp ctrlm switchm |} <+>  sws)  links ->
-    LinksHaveDst 
-      ({| Switch swId pts tbl' inp' outp' ctrlm' switchm' |} <+> sws)
-      links.
-  Proof with auto.
-
-    intros.
-    unfold LinksHaveDst in *.
-    intros.
-    apply H in H0. clear H.
-    unfold LinkHasDst in *.
-    destruct H0 as [sw [HMem [HEq HIn]]].
-    simpl in HMem.
-    rewrite -> Bag.in_union in HMem.
-    destruct HMem.
-    + destruct sw.
-      simpl in *.
-      destruct H.
-      inversion H.
-      subst.
-      eexists.
-      split. 
-      apply Bag.in_union. left. simpl. left. reflexivity.
-      simpl...
-      inversion H.
-    + exists sw.
-      split...
-      simpl...
-      apply Bag.in_union...
-  Qed.
-
-   Lemma LinkTopoOK_inv : forall {links links0 src dst} pks pks',
-     ConsistentDataLinks (links ++ (DataLink src pks dst) :: links0) ->
-     ConsistentDataLinks (links ++ (DataLink src pks' dst) :: links0).
-   Proof with auto with datatypes.
-     intros.
-     unfold ConsistentDataLinks in *.
-     intros.
-     apply in_app_iff in H0.
-     simpl in H0.
-     destruct H0 as [H0 | [H0 | H0]]...
-     pose (lnk' := (DataLink src0 pks0 dst0)).
-     remember (H lnk').
-     assert (In lnk' (links0 ++ lnk' :: links1))...
-     apply e in H1.
-     simpl in H1.
-     inversion H0.
-     simpl...
-   Qed.
-
-
-  Lemma FlowTablesSafe_untouched : forall {sws swId pts tbl inp inp'
-    outp outp' ctrlm ctrlm' switchm switchm' },
-    FlowTablesSafe
-      ({|Switch swId pts tbl inp outp ctrlm switchm|} <+> sws) ->
-    FlowTablesSafe 
-      ({|Switch swId pts tbl inp' outp' ctrlm' switchm'|} <+> sws).
-  Proof with eauto.
-    intros.
-    unfold FlowTablesSafe in *.
-    intros.
-    simpl in H0.
-    apply Bag.in_union in H0.
-    destruct H0.
-    + inversion H0.
-      inversion H1.
-      subst.
-      eapply H. simpl. apply Bag.in_union. left. simpl. left...
-      simpl in H1; inversion H1.
-    + eapply H. apply Bag.in_union. right...
-  Qed.
-
-  Lemma LinksHaveSrc_inv : forall {sws links links0 src dst} pks pks',
-    LinksHaveSrc sws (links ++ (DataLink src pks dst) :: links0) ->
-    LinksHaveSrc sws (links ++ (DataLink src pks' dst) :: links0).
-  Proof with auto with datatypes.
-    intros.
-    unfold LinksHaveSrc in *.
-    intros.
-    apply in_app_iff in H0.
-    simpl in H0.
-    destruct H0 as [H0 | [H0 | H0]]; subst...
-    destruct (H (DataLink src0 pks0 dst0))...
-    destruct H0 as [HMem [HEq HIn]].
-    simpl in *.
-    unfold LinkHasSrc.
-    exists x...
-  Qed.
-
-  Lemma LinksHaveDst_inv : forall {sws links links0 src dst} pks pks',
-    LinksHaveDst sws (links ++ (DataLink src pks dst) :: links0) ->
-    LinksHaveDst sws (links ++ (DataLink src pks' dst) :: links0).
-  Proof with auto with datatypes.
-    intros.
-    unfold LinksHaveDst in *.
-    intros.
-    apply in_app_iff in H0.
-    simpl in H0.
-    destruct H0 as [H0 | [H0 | H0]]; subst...
-    destruct (H (DataLink src0 pks0 dst0))...
-    destruct H0 as [HMem [HEq HIn]].
-    simpl in *.
-    unfold LinkHasDst.
-    exists x...
-  Qed.
-
-  Lemma UniqSwIds_pres : forall {sws swId pts tbl inp outp ctrlm switchm
-    pts' tbl' inp' outp' ctrlm' switchm'},
-    UniqSwIds ({|Switch swId pts tbl inp outp ctrlm switchm|} <+> sws) ->
-    UniqSwIds ({|Switch swId pts' tbl' inp' outp' ctrlm' switchm'|} <+> sws).
-  Proof with auto with datatypes.
-    intros.
-    unfold UniqSwIds in *.
-    unfold union in H.
-    unfold to_list in H.
-    simpl in H.
-    destruct sws.
-    rename to_list into swsLst.
-    unfold union.
-    unfold to_list.
-    simpl.
-    (* might need induction (shouldn't since swId is the same *)
-  Admitted.
-
-  Lemma OfLinksHaveSrc_pres1 : forall { sws swId pts1 tbl1 inp1 outp1 ctrlm1 
-    switchm1 pts2 tbl2 inp2 outp2 ctrlm2 switchm2 switchmLst1 ctrlmLst1
-    switchmLst2 ctrlmLst2 ofLinks1 ofLinks2 },
-    OFLinksHaveSw
-      ({|Switch swId pts1 tbl1 inp1 outp1 ctrlm1 switchm1|} <+> sws)
-      (ofLinks1 ++ OpenFlowLink swId switchmLst1 ctrlmLst1 :: ofLinks2) ->
-    OFLinksHaveSw
-      ({|Switch swId pts2 tbl2 inp2 outp2 ctrlm2 switchm2|} <+> sws)
-      (ofLinks1 ++ OpenFlowLink swId switchmLst2 ctrlmLst2 :: ofLinks2).
-  Proof with auto with datatypes.
-    intros.
-    unfold OFLinksHaveSw in *.
-    intros.
-    destruct ofLink.
-    unfold ofLinkHasSw in *.
-    apply in_app_iff in H0; simpl in H0; destruct H0 as [H0 | [H0 | H0]]; subst.
-    + destruct H with (ofLink := OpenFlowLink of_to0 of_switchm0 of_ctrlm0)
-        as [sw [HMem HEq]]...
-      assert ({ of_to0 = swId0 } + { of_to0 <> swId0 }) as J by (apply TotalOrder.eqdec).
-      destruct J; subst.
-      - exists (Switch swId0 pts2 tbl2 inp2 outp2 ctrlm2 switchm2).
-        split...
-        apply Bag.in_union.
-        left.
-        simpl...
-      - exists sw.
-        destruct sw.
-        simpl in HEq.
-        subst.
-        split...
-        apply Bag.in_union.
-        right.
-        apply Bag.in_union in HMem.
-        destruct HMem.
-        * simpl in H1.
-          destruct H1.
-          inversion H1.
-          subst.
-          contradiction n...
-          inversion H1.
-        * trivial.
-    + inversion H0; subst; clear H0.
-      exists (Switch of_to0 pts2 tbl2 inp2 outp2 ctrlm2 switchm2).
-      split...
-      apply Bag.in_union.
-      left.
-      simpl...
-    + destruct H with (ofLink := OpenFlowLink of_to0 of_switchm0 of_ctrlm0) 
-        as [sw [HMem HEq]]...
-      assert ({ of_to0 = swId0 } + { of_to0 <> swId0 }) as J by (apply TotalOrder.eqdec).
-      destruct J; subst.
-      - exists (Switch swId0 pts2 tbl2 inp2 outp2 ctrlm2 switchm2).
-        split... apply Bag.in_union. left. simpl...
-      - exists sw.
-        destruct sw.
-        simpl in HEq.
-        subst.
-        split...
-        apply Bag.in_union.
-        right.
-        apply Bag.in_union in HMem.
-        destruct HMem...
-        simpl in H1.
-        destruct H1.
-        * inversion H1.
-          subst.
-          contradiction n...
-        * inversion H1.
-  Qed.
-
-  Lemma OfLinksHaveSrc_pres2 : forall { sws swId pts1 tbl1 inp1 outp1 ctrlm1 
-    switchm1 pts2 tbl2 inp2 outp2 ctrlm2 switchm2 ofLinks },
-    OFLinksHaveSw
-      ({|Switch swId pts1 tbl1 inp1 outp1 ctrlm1 switchm1|} <+> sws)
-      ofLinks ->
-    OFLinksHaveSw
-      ({|Switch swId pts2 tbl2 inp2 outp2 ctrlm2 switchm2|} <+> sws)
-      ofLinks.
-  Proof with auto with datatypes.
-    intros.
-    unfold OFLinksHaveSw in *.
-    intros.
-    destruct ofLink.
-    apply H in H0.
-    clear H.
-    unfold ofLinkHasSw in *.
-    destruct H0 as [sw [HMem HEq]].
-    simpl in HEq.
-    destruct sw.
-    assert ({ of_to0 = swId0 } + { of_to0 <> swId0 }) as J by (apply TotalOrder.eqdec).
-    destruct J; subst.
-    simpl in *. subst.
-    exists (Switch swId0 pts2 tbl2 inp2 outp2 ctrlm2 switchm2).
-    split... 
-    + apply Bag.in_union.
-      left.
-      simpl...
-    + exists (Switch swId1 pts0 tbl0 inp0 outp0 ctrlm0 switchm0).
-      apply Bag.in_union in HMem.
-      destruct HMem.
-      - simpl in H.
-        destruct H.
-        * inversion H.
-          subst.
-          simpl in n.
-          contradiction n...
-        * inversion H.
-      - split...
-        apply Bag.in_union...
-  Qed.
-
-  Lemma OfLinksHaveSrc_pres3 : forall { sws swId switchmLst1 ctrlmLst1
-    switchmLst2 ctrlmLst2 ofLinks1 ofLinks2 },
-    OFLinksHaveSw sws
-      (ofLinks1 ++ OpenFlowLink swId switchmLst1 ctrlmLst1 :: ofLinks2) ->
-    OFLinksHaveSw sws
-      (ofLinks1 ++ OpenFlowLink swId switchmLst2 ctrlmLst2 :: ofLinks2).
-  Proof with auto with datatypes.
-    intros.
-    unfold OFLinksHaveSw in *.
-    intros.
-    destruct ofLink.
-    apply in_app_iff in H0; simpl in H0; destruct H0 as [H0 | [H0 | H0]]; subst...
-    inversion H0; subst; clear H0.
-    unfold ofLinkHasSw in *.
-    destruct (H (OpenFlowLink of_to0 switchmLst1 ctrlmLst1)) as [sw [HMem HEq]]...
-    exists sw...
-  Qed.
+  Module Import Lemmas := FwOF.FwOFWellFormednessLemmas.Make (RelationDefinitions).
 
   Hint Resolve OfLinksHaveSrc_pres1 OfLinksHaveSrc_pres2 OfLinksHaveSrc_pres3.
-
-  Section FMS.
-
-    Hint Constructors FMS SafeWire SwitchEP.
-
-    Hint Resolve FMS_untouched.
-
-    Lemma SwitchEP_equiv : forall swId pts tbl inp0 inp1 outp0 outp1
-      ctrlm0 switchm0 switchm1 ep,
-      SwitchEP (Switch swId pts tbl inp0 outp0 ctrlm0 switchm0) ep ->
-      SwitchEP (Switch swId pts tbl inp1 outp1 ctrlm0 switchm1) ep.
-    Proof with eauto.
-      intros.
-      inversion H; subst.
-      apply NoFlowModsInBuffer...
-      eapply OneFlowModInBuffer...
-    Qed.
-
-    Lemma AllFMS_untouched1 : forall swId0 pts0 tbl0 inp0 outp0 ctrlm0 switchm0
-      inp1 outp1 switchm1 sws ofLinks0,
-      AllFMS ({|Switch swId0 pts0 tbl0 inp0 outp0 ctrlm0 switchm0|} <+> sws)
-             ofLinks0 ->
-      AllFMS ({|Switch swId0 pts0 tbl0 inp1 outp1 ctrlm0 switchm1|} <+> sws)
-             ofLinks0.
-    Proof with simpl;eauto.
-      intros.
-      unfold AllFMS.
-      intros.
-      apply Bag.in_union in H0.
-      destruct H0 as [H0 | H0].
-      + destruct sw.
-        simpl in H0.
-        destruct H0 as [H0 | H0].
-        2: solve[inversion H0].
-        inversion H0.
-        subst. 
-        clear H0.
-        assert (In (Switch swId1 pts1 tbl1 inp0 outp0 ctrlm1 switchm0)
-                  (to_list ({|(Switch swId1 pts1 tbl1 inp0 outp0 ctrlm1 switchm0)|} <+>
-                   sws))) as J.
-        { apply Bag.in_union... }
-        apply H in J.
-        simpl in J.
-        destruct J as [lnk [HIn [HEq FMSsw0]]].
-        simpl.
-        exists lnk.
-        split...
-        split...
-        remember FMSsw0 as FMSorig eqn:X; clear X.
-        inversion FMSsw0. 
-        clear HEq.
-        subst.
-        eapply MkFMS...
-        eapply SwitchEP_equiv...
-      +  assert (In sw
-                   (to_list ({|Switch swId0 pts0 tbl0 inp0 outp0 ctrlm0 switchm0|} <+> sws)))
-             as X...
-         apply Bag.in_union...
-    Qed.
-
-  End FMS.
-
   Hint Unfold UniqSwIds.
-  Hint Resolve step_preserves_P.
-
-  Section DevicesFromTopo.
-    
-    Hint Unfold DevicesFromTopo.
-
-    Lemma DevicesFromTopo_pres0 : forall swId0 pts0 tbl0 inp0 outp0 ctrlm0
-      switchm0 pts1 tbl1 inp1 outp1 ctrlm1 switchm1 sws links0 ofLinks0
-      ctrl0,
-      DevicesFromTopo
-        (State ({|Switch swId0 pts0 tbl0 inp0 outp0 ctrlm0 switchm0|} <+> sws)
-               links0
-               ofLinks0
-               ctrl0) ->
-      DevicesFromTopo
-        (State ({|Switch swId0 pts1 tbl1 inp1 outp1 ctrlm1 switchm1|} <+> sws)
-               links0
-               ofLinks0
-               ctrl0).
-    Proof with simpl; eauto.
-      intros.
-      unfold DevicesFromTopo in *.
-      intros.
-      apply H in H0.
-      clear H.
-      destruct H0 as [sw0 [sw1 [lnk [HMemSw0 [HMemSw1 [HInLnk [HSw0Eq [HSw1Eq
-                     [HLnkSrcEq HLnkDstEq]]]]]]]]].
-      destruct lnk.
-      simpl in *.
-      destruct sw0.
-      destruct sw1.
-      simpl in *.
-      subst.
-      apply Bag.in_union in HMemSw0.
-      apply Bag.in_union in HMemSw1.
-      destruct HMemSw0; destruct HMemSw1.
-      + eexists. eexists. eexists.
-        simpl in H; simpl in H0.
-        destruct H0; destruct H...
-        inversion H; inversion H0...
-        subst...
-        subst...
-        split...
-        apply Bag.in_union.
-        left...
-        split...
-        apply  Bag.in_union. left...
-        split...
-        inversion H.
-        inversion H0.
-        inversion H.
-      + do 3 eexists.
-        simpl in H.
-        destruct H. 2: solve[inversion H].
-        inversion H. subst.
-        repeat split.
-        apply Bag.in_union. left. simpl. left. reflexivity.
-        apply Bag.in_union. right. exact H0.
-        exact HInLnk.
-        trivial.
-        trivial.
-        trivial.
-        trivial.
-      + do 3 eexists.
-        simpl in H0.
-        destruct H0. 2: solve[inversion H0].
-        inversion H0; subst; clear H0.
-        repeat split...
-        apply Bag.in_union. right. exact H.
-        apply Bag.in_union. left. simpl. left. reflexivity.
-        trivial.
-        trivial.
-      + do 3 eexists.
-        repeat split...
-        apply Bag.in_union. right. exact H.
-        apply Bag.in_union. right. exact H0.
-        trivial.
-        trivial.
-    Qed.
-
-    Lemma DevicesFromTopo_pres1 : forall sws0 links0 links1 src
-      dst pks0 pks1 ofLinks0 ctrl0,
-      DevicesFromTopo
-        (State sws0
-               (links0 ++ DataLink src pks0 dst :: links1)
-               ofLinks0
-               ctrl0) ->
-      DevicesFromTopo
-        (State sws0
-               (links0 ++ DataLink src pks1 dst :: links1)
-               ofLinks0
-               ctrl0).
-    Proof with simpl; eauto with datatypes.
-      intros.
-      unfold DevicesFromTopo in *.
-      intros.
-      apply H in H0.
-      clear H.
-      destruct H0 as [sw0 [sw1 [lnk [HMemSw0 [HMemSw1 [HInLnk [HSw0Eq [HSw1Eq
-                     [HLnkSrcEq HLnkDstEq]]]]]]]]].
-      destruct lnk.
-      simpl in *.
-      destruct sw0.
-      destruct sw1.
-      simpl in *.
-      subst.
-      rewrite -> in_app_iff in HInLnk. simpl in HInLnk.
-      destruct HInLnk as [HInLnk | [HInLnk | HInLnk]].
-      + repeat eexists.
-        exact HMemSw0.
-        exact HMemSw1.
-        instantiate (1 := DataLink (swId1,pt1) pks2 (swId0,pt0)).
-        auto with datatypes.
-        simpl...
-        simpl...
-        simpl...
-        simpl...
-      + repeat eexists.
-        exact HMemSw0.
-        exact HMemSw1.
-        instantiate (1 := DataLink (swId1,pt1) pks1 (swId0,pt0)).
-        inversion HInLnk. subst.
-        auto with datatypes.
-        simpl...
-        simpl...
-        simpl...
-        simpl...
-      + repeat eexists.
-        exact HMemSw0.
-        exact HMemSw1.
-        instantiate (1 := DataLink (swId1,pt1) pks2 (swId0,pt0)).
-        auto with datatypes.
-        simpl...
-        simpl...
-        simpl...
-        simpl...
-    Qed.
-        
-  End DevicesFromTopo.
-
-  Section SwitchesHaveOpenFlowLinks.
-    
-    Hint Unfold SwitchesHaveOpenFlowLinks.
-
-    Lemma SwitchesHaveOpenFlowLinks_pres0 : forall swId0 pts0 tbl0 inp0 outp0 
-      ctrlm0 switchm0 pts1 tbl1 inp1 outp1 ctrlm1 switchm1 sws links0 ofLinks0
-      ctrl0,
-      SwitchesHaveOpenFlowLinks
-        (State ({|Switch swId0 pts0 tbl0 inp0 outp0 ctrlm0 switchm0|} <+> sws)
-               links0
-               ofLinks0
-               ctrl0) ->
-      SwitchesHaveOpenFlowLinks
-        (State ({|Switch swId0 pts1 tbl1 inp1 outp1 ctrlm1 switchm1|} <+> sws)
-               links0
-               ofLinks0
-               ctrl0).
-    Proof with simpl; eauto.
-      intros.
-      unfold SwitchesHaveOpenFlowLinks in *.
-      intros.
-      simpl in *.
-      apply Bag.in_union in H0.
-      simpl in H0.
-      destruct H0 as [[H0 | H0] | H0].
-      + destruct sw.
-        inversion H0; subst; clear H0.
-        apply H.
-        apply Bag.in_union.
-        (*
-      + assert ( (Switch swId0 pts0 tbl0 inp0 outp0 ctrlm0 switchm0)  === (Switch swId0 pts0 tbl0 inp0 outp0 ctrlm0 switchm0) \/ Mem (Switch swId0 pts0 tbl0 inp0 outp0 ctrlm0 switchm0) sws).
-        left. apply reflexivity.
-        apply H in H1. clear H.
-        destruct H1 as [ofLink [HIn HSwEq]].
-        destruct ofLink.
-        simpl in *.
-        subst.
-        inversion H0; subst.
-        eexists...
-      + destruct (H sw (or_intror H0)) as [ofLink [HIn HSwEq]].
-        destruct ofLink.
-        simpl in *.
-        subst.
-        destruct sw.
-        simpl in *.
-        subst.
-        eexists... *)
-    Admitted.
-
-    Lemma SwitchesHaveOpenFlowLinks_pres1 : forall sws0 links0 ofLinks0
-      ofLinks1 swId switchm0 ctrlm0 switchm1 ctrlm1
-      ctrl0,
-      SwitchesHaveOpenFlowLinks
-        (State sws0 links0
-               (ofLinks0 ++ OpenFlowLink swId switchm0 ctrlm0 :: ofLinks1)
-               ctrl0) ->
-      SwitchesHaveOpenFlowLinks
-        (State sws0 links0
-               (ofLinks0 ++ OpenFlowLink swId switchm1 ctrlm1 :: ofLinks1)
-               ctrl0).
-      Proof with eauto with datatypes.
-        unfold SwitchesHaveOpenFlowLinks.
-        intros.
-        simpl in *.
-        apply H in H0.
-        clear H.
-        destruct H0 as [ofLink [HIn HIdEq]].
-        apply in_app_iff in HIn.
-        simpl in HIn.
-        destruct HIn as [HIn | [HIn | HIn]].
-        + eexists...
-        + exists (OpenFlowLink swId0 switchm1 ctrlm1).
-          split...
-          subst.
-          simpl in *...
-        + eexists...
-      Qed.
-        
-  End SwitchesHaveOpenFlowLinks.
-
+  Hint Resolve P_entails_FlowTablesSafe step_preserves_P.
   Hint Resolve DevicesFromTopo_pres0 DevicesFromTopo_pres1 SwitchesHaveOpenFlowLinks_pres0
        SwitchesHaveOpenFlowLinks_pres1.
+  Hint Resolve LinksHaveSrc_untouched.
+  Hint Resolve LinksHaveDst_untouched.
+  Hint Resolve FlowTablesSafe_untouched.
+  Hint Resolve UniqSwIds_pres.
+  Hint Resolve FlowTablesSafe_PacketOut.
+  Hint Resolve AllDiff_preservation.
+
+  Ltac sauto := solve[eauto with datatypes].
 
   Lemma simpl_step : forall (st1 st2 : state) obs
     (tblsOk1 : FlowTablesSafe (switches st1))
@@ -724,42 +39,38 @@ Module Make (AtomsAndController_ : ATOMS_AND_CONTROLLER) <: RELATION.
     (haveSrc1 : LinksHaveSrc (switches st1) (links st1))
     (haveDst1 : LinksHaveDst (switches st1) (links st1))
     (uniqSwIds1 : UniqSwIds (switches st1))
-    (allFMS1 : AllFMS (switches st1) (ofLinks st1))
     (P0 : P (switches st1) (ofLinks st1) (ctrl st1))
     (uniqOfLinkIds1 : AllDiff of_to (ofLinks st1))
     (ofLinksHaveSw1 : OFLinksHaveSw (switches st1) (ofLinks st1))
     (devsFromTopo1 : DevicesFromTopo st1)
-    (swsHaveOFLinks1 : SwitchesHaveOpenFlowLinks st1),
+    (swsHaveOFLinks1 : SwitchesHaveOpenFlowLinks (switches st1) (ofLinks st1)),
     step st1 obs st2 ->
-    exists tblsOk2 linksTopoOk2 haveSrc2 haveDst2 uniqSwIds2 allFMS2 P1
+    exists tblsOk2 linksTopoOk2 haveSrc2 haveDst2 uniqSwIds2 P1
            uniqOfLinkIds2 ofLinksHaveSw2 devsFromTopo2 swsHaveOFLinks2,
       concreteStep
         (ConcreteState st1 tblsOk1 linksTopoOk1 haveSrc1 haveDst1 uniqSwIds1
-                       allFMS1 P0 uniqOfLinkIds1 ofLinksHaveSw1 devsFromTopo1
+                       P0 uniqOfLinkIds1 ofLinksHaveSw1 devsFromTopo1
                        swsHaveOFLinks1)
         obs
         (ConcreteState st2 tblsOk2 linksTopoOk2 haveSrc2 haveDst2 uniqSwIds2
-                       allFMS2 P1 uniqOfLinkIds2 ofLinksHaveSw2 devsFromTopo2
+                       P1 uniqOfLinkIds2 ofLinksHaveSw2 devsFromTopo2
                        swsHaveOFLinks2).
-  Proof with eauto with datatypes.
+  Proof with simpl;eauto with datatypes.
     intros.
     unfold concreteStep.
     simpl.
-    { inversion H; subst.
+    { inversion H; subst; simpl in *.
       (* Case 1. *)
-      + exists (FlowTablesSafe_untouched tblsOk1).
-        exists linksTopoOk1.
-        exists (LinksHaveSrc_untouched haveSrc1).
-        exists (LinksHaveDst_untouched haveDst1).
-        exists (UniqSwIds_pres uniqSwIds1).
-        exists (AllFMS_untouched1 _ _ _ allFMS1).
-        eexists. simpl...
-        eexists. simpl...
-        exists (OfLinksHaveSrc_pres2 ofLinksHaveSw1).
+      + eexists...
+        eexists...
+        eexists...
+        eexists...
+        eexists...
+        eexists...
+        eexists...
         eexists...
       (* Case 2: processed a buffered FlowMod *)
-      + simpl in *.
-        eexists.
+      + eexists.
         unfold FlowTablesSafe.
         intros.
         apply Bag.in_union in H0. simpl in H0.
@@ -767,439 +78,161 @@ Module Make (AtomsAndController_ : ATOMS_AND_CONTROLLER) <: RELATION.
           [idtac | solve[inversion HContra] | idtac].
           (* interesting case, where the flow table has been modified *)
           - inversion HIn; subst; clear HIn.
-            unfold AllFMS in allFMS1.
-            edestruct allFMS1 as [lnk0 [HLnkIn [HEq HFMS]]].
-            { apply Bag.in_union. left. simpl. left. reflexivity. }
-            destruct lnk0; simpl in *; subst.
-            inversion HFMS; subst.
-            inversion H2; subst.
+            assert (FlowModSafe swId1 tbl0 (({|FlowMod fm|}) <+> ctrlm1)) as J.
+            { unfold FlowTablesSafe in tblsOk1.
+              eapply tblsOk1.
+              apply Bag.in_union. left. simpl... }
+            inversion J; subst.
             * assert (NotFlowMod (FlowMod fm)) as Hcontra.
-              { apply H9. apply Bag.in_union. left. simpl... }
+              { apply H0. apply Bag.in_union; simpl... }
               inversion Hcontra.
-            * assert (In (FlowMod fm) (to_list (({|FlowMod f|}) <+> ctrlm2))) 
-                as X.
-              { rewrite <- H11. apply Bag.in_union. left. simpl... }
-              apply Bag.in_union in X. simpl in X.
-              { destruct X as [[X | X] | X].
-                + inversion X; subst...
-                + inversion X.
-                + apply H9 in X. inversion X. }
+            * assert (f = fm /\ ctrlm0 = ctrlm1) as HEq.
+              admit. (* obvious *)
+              destruct HEq; subst...
+              apply NoFlowModsInBuffer...
           - unfold FlowTablesSafe in tblsOk1.
             eapply tblsOk1.
-            apply Bag.in_union. right. exact HIn. }
+            apply Bag.in_union... } 
         eexists...
-        exists (LinksHaveSrc_untouched haveSrc1).
-        exists (LinksHaveDst_untouched haveDst1).
-        exists (UniqSwIds_pres uniqSwIds1).
-        eexists.
-        { unfold AllFMS.
-          intros.
-        apply Bag.in_union in H0; simpl in H0.
-        { destruct H0 as [[HIn | HContra] | HIn]; 
-          [idtac | solve[inversion HContra] | idtac].
-          (* interesting case, where the flow table has been modified *)
-          - subst.
-            unfold AllFMS in allFMS1.
-            edestruct allFMS1 as [lnk0 [HLnkIn [HEq HFMS]]].
-            { apply Bag.in_union. left. simpl. left. reflexivity. }
-            exists lnk0.
-            destruct lnk0; simpl in *; subst.
-            repeat split...
-            inversion HFMS; subst.
-            inversion H2; subst.
-            * assert (NotFlowMod (FlowMod fm)) as Hcontra.
-              { apply H9. apply Bag.in_union. left. simpl... }
-              inversion Hcontra.
-            * assert (In (FlowMod fm) (to_list (({|FlowMod f|}) <+> ctrlm2))) 
-                as X.
-              { rewrite <- H11. apply Bag.in_union. left. simpl... }
-              apply Bag.in_union in X. simpl in X.
-              { destruct X as [[X | X] | X].
-                + inversion X; subst.
-                  rewrite <- Bag.pop_union_l in H11.
-                  destruct H10 as [ctrlEp Hsafewire].
-                  eapply MkFMS. 
-                  eapply NoFlowModsInBuffer.
-                  intros...
-                  apply H9.
-                  rewrite <- H11...
-                  instantiate (1:= (Endpoint_NoBarrier (modify_flow_table fm tbl0)))...
-                  exists ctrlEp...
-                + inversion X.
-                + apply H9 in X. inversion X. }
-          - subst.
-            unfold AllFMS in allFMS1.
-            edestruct allFMS1 as [lnk0 [HLnkIn [HEq HFMS]]].
-            { apply Bag.in_union. right. exact HIn. }
-            exists lnk0... } }
-        eexists. simpl...
-        eexists. simpl...
-        exists (OfLinksHaveSrc_pres2 ofLinksHaveSw1).
         eexists...
-      (* Case 4. *)
-      + exists (FlowTablesSafe_untouched tblsOk1).
-        exists linksTopoOk1.
-        exists (LinksHaveSrc_untouched haveSrc1).
-        exists (LinksHaveDst_untouched haveDst1).
-        exists (UniqSwIds_pres uniqSwIds1).
-        simpl in *.
-        eexists.
-        unfold AllFMS.
-        intros.
-        destruct sw.
-        simpl in *.
-        { apply Bag.in_union in H1. simpl in H1.
-          { destruct H1 as [[H1 | HContra] | H1]; 
-            [idtac | solve[inversion HContra] | idtac].
-          + inversion H1.
-            subst.
-            unfold AllFMS in allFMS1.
-            edestruct allFMS1 as [lnk0 [HLnkIn [HEq HFMS]]].
-            apply Bag.in_union. left. simpl. left. reflexivity.
-            simpl in HEq.
-            subst.
-            exists lnk0.
-            split...
-            split...
-            destruct lnk0.
-            simpl.
-            simpl in *.
-            apply FMS_dequeue_pktOut...
-          + unfold AllFMS in allFMS1.
-            simpl in allFMS1.
-            apply (allFMS1 (Switch swId1 pts1 tbl1 inp1 outp1 ctrlm1 
-                                   switchm1))...
-            apply Bag.in_union.
-            right... } }
+        eexists...
+        eexists...
         eexists...
         eexists...
         eexists...
+      (* Case 4. *)
+      + eexists. sauto.
+        eexists. sauto.
+        eexists. sauto.
+        eexists. sauto.
+        eexists. sauto.
+        eexists. sauto.
+        eexists. sauto.
+        eexists. sauto.
+        eexists. sauto.
+        eexists. sauto.
+        sauto.
       (* Case 5. *)
-      + exists (FlowTablesSafe_untouched tblsOk1).
+      + eexists. sauto.
         exists (LinkTopoOK_inv pks0 (pk::pks0) linksTopoOk1).
         exists (LinksHaveSrc_inv pks0 (pk::pks0) (LinksHaveSrc_untouched haveSrc1)).
         exists (LinksHaveDst_inv pks0 (pk::pks0) (LinksHaveDst_untouched haveDst1)).
-        exists (UniqSwIds_pres uniqSwIds1).
-        exists (AllFMS_untouched1 _ _ _ allFMS1).
-        eexists. eauto.
-        eexists. eauto.
-        eexists. simpl. eauto.
-        eexists...
+        eexists. sauto.
+        eexists. sauto.
+        eexists. sauto.
+        eexists. sauto.
+        eexists. sauto.
+        eexists. sauto.
+        sauto.
       (* Case 6. *)
-      + exists (FlowTablesSafe_untouched tblsOk1).
+      + eexists. sauto.
         exists (LinkTopoOK_inv (pks0 ++ [pk]) pks0 linksTopoOk1).
         exists 
           (LinksHaveSrc_inv (pks0 ++ [pk]) pks0 (LinksHaveSrc_untouched haveSrc1)).
         exists 
           (LinksHaveDst_inv (pks0 ++ [pk]) pks0 (LinksHaveDst_untouched haveDst1)).
-        exists (UniqSwIds_pres uniqSwIds1).
-        exists (AllFMS_untouched1 _ _ _ allFMS1).
-        eexists...
-        exists. simpl...
-        exists. simpl...
-        eauto.
-        eexists...
+        eexists. sauto.
+        eexists. sauto.
+        eexists. sauto.
+        eexists. sauto.
+        eexists. sauto.
+        eexists. sauto.
+        sauto.
       (* Case 7. *)
-      + exists tblsOk1.
-        exists linksTopoOk1.
-        exists haveSrc1.
-        exists haveDst1.
-        exists uniqSwIds1.
-        exists allFMS1.
-        eexists...
+      + eexists. sauto.
+        eexists. sauto.
+        eexists. sauto.
+        eexists. sauto.
+        eexists. sauto.
+        eexists. sauto.
+        eexists. sauto.
+        eexists. sauto.
+        eexists. sauto.
+        eexists. sauto.
+        sauto.
       (* Case 8. *)
-      + simpl in *.
-        exists tblsOk1.
-        exists linksTopoOk1.
-        exists haveSrc1.
-        exists haveDst1.
-        exists uniqSwIds1.
-        eexists.
-        unfold AllFMS in *. intros. destruct sw. subst.
-        assert ({swId0 = swId1 } + { swId0 <> swId1 }) as HIdEq.
-        { apply TotalOrder.eqdec. }
-        { destruct HIdEq; subst.
-          + exists (OpenFlowLink swId1 fromSwitch0 fromCtrl).
-            split...
-            split...
-            destruct (allFMS1 (Switch swId1 pts0 tbl0 inp0 outp0 ctrlm0 switchm0)) as [lnk [HLnkIn [HId HFMS]]].
-            { auto. }
-            destruct lnk.
-            simpl in *.
-            subst.
-            assert (OpenFlowLink swId1 of_switchm0 of_ctrlm0 =
-                    OpenFlowLink swId1 (fromSwitch0 ++ [msg]) fromCtrl) as HOfEq.
-            { eapply AllDiff_uniq... }
-            inversion HOfEq; subst; clear HOfEq.
-            apply FMS_untouched with (inp0 := inp0) (outp0 := outp0) (switchm0 := switchm0)
-                                                    (switchmLst0 := fromSwitch0 ++ [msg]).
-            exact HFMS.
-          + destruct (allFMS1 (Switch swId1 pts0 tbl0 inp0 outp0 ctrlm0 switchm0)) as [lnk [HLnkIn [HId HFMS]]].
-            { simpl. exact H1. }
-            exists lnk.
-            apply in_app_iff in HLnkIn.
-            simpl in HLnkIn.
-            { destruct HLnkIn as [HLnkIn | [HLnkIn | HLnkIn]].
-              + split...
-              + destruct lnk. inversion HLnkIn. contradiction n. subst...
-              + split... } }
-        exists...
-        exists. eapply AllDiff_preservation. exact uniqOfLinkIds1.
-          do 2 rewrite -> map_app...
-        exists (OfLinksHaveSrc_pres3 ofLinksHaveSw1).
-        eauto.
+      + eexists. sauto.
+        eexists. sauto.
+        eexists. sauto.
+        eexists. sauto.
+        eexists. sauto.
+        eexists. sauto.
+        eexists. 
+        { eapply AllDiff_preservation.
+          exact uniqOfLinkIds1.
+          do 2 rewrite -> map_app... }
+        eexists. sauto.
+        eexists. sauto.
+        eexists. sauto.
+        sauto.
       (* Case 9. *)
-      + simpl in *.
-        exists tblsOk1.
-        exists linksTopoOk1.
-        exists haveSrc1.
-        exists haveDst1.
-        exists uniqSwIds1.
+      + eexists. sauto.
+        eexists. sauto.
+        eexists. sauto.
+        eexists. sauto.
+        eexists. sauto.
+        eexists. sauto.
         eexists.
-        unfold AllFMS.
-        simpl in *.
-        intros.
-        unfold AllFMS in allFMS1.
-        destruct (allFMS1 _ H1) as [lnk [HIn [HLnkIdEq HFMS]]].
-        apply in_app_iff in HIn; simpl in HIn.
-        { destruct HIn as [HIn | [HIn | HIn]].
-        * exists lnk; auto with datatypes.
-        * exists (OpenFlowLink swId0 fromSwitch0 (msg :: fromCtrl)).
-          split...
-          split; subst...
-          simpl in *.
-          destruct sw.
-          subst.
-          inversion HFMS; subst.
-          inversion H4; subst.
-          simpl in *.
-          - eapply MkFMS...
-            destruct H12 as [ctrlEp0 HSafeWire].
-            destruct (ControllerFMS _ _ _ HSafeWire P0 H0 H H1 H4) as [ctrlEp1 HSafeWire1]...
-          - eapply MkFMS...
-            destruct H12 as [ctrlEp0 HSafeWire].
-            destruct (ControllerFMS _ _ _ HSafeWire P0 H0 H H1 H4) as [ctrlEp1 HSafeWire1]...
-        * exists lnk; auto with datatypes. }
-        exists...
-        exists. eapply AllDiff_preservation. exact uniqOfLinkIds1.
-          simpl. do 2 rewrite -> map_app...
-        exists. simpl. eauto.
-        eauto.
+        { eapply AllDiff_preservation.
+          exact uniqOfLinkIds1.
+          do 2 rewrite -> map_app... }
+        eexists. sauto.
+        eexists. sauto.
+        eexists. sauto.
+        sauto.
       (* Case 10. *)
-      + simpl in *.
-        exists (FlowTablesSafe_untouched tblsOk1).
-        exists linksTopoOk1.
-        exists (LinksHaveSrc_untouched haveSrc1).
-        exists (LinksHaveDst_untouched haveDst1).
-        exists (UniqSwIds_pres uniqSwIds1).
+      + eexists. sauto.
+        eexists. sauto.
+        eexists. sauto.
+        eexists. sauto.
+        eexists. sauto.
+        eexists. sauto.
         eexists.
-        unfold AllFMS in *.
-        intros.
-        destruct sw.
-        subst.
-        assert ({swId0 = swId1 } + { swId0 <> swId1 }) as HIdEq.
-        { apply TotalOrder.eqdec. }
-        { destruct HIdEq; subst.
-          + unfold UniqSwIds in uniqSwIds1. (* Not what we want, since it has {|msg|} *)
-            assert (AllDiff swId (to_list 
-                                    (({|Switch swId1 pts0 tbl0 inp0 outp0 ctrlm0 switchm0|}) <+> sws))) as uniqSwIds2.
-            { eapply Bag.AllDiff_preservation... }
-            exists (OpenFlowLink swId1 (msg :: fromSwitch0) fromCtrl).
-            split...
-            split...
-            destruct (allFMS1 (Switch swId1 pts0 tbl0 inp0 outp0 ctrlm0 ({|msg|} <+> switchm0))) as [lnk J].
-            { simpl. apply Bag.in_union. left. simpl. left. trivial. }
-            destruct J as [HLnkIn [HId HFMS]].
-            simpl in HId.
-            destruct lnk.
-            subst.
-            simpl in *.
-            assert (OpenFlowLink of_to0 of_switchm0 of_ctrlm0 =
-                    OpenFlowLink of_to0 fromSwitch0 fromCtrl) as HEqOf.
-            { eapply AllDiff_uniq... }
-            inversion HEqOf; subst; clear HEqOf.
-            apply FMS_untouched 
-              with (inp0 := inp0) (outp0 := outp0) 
-                   (switchm0 := ({|msg|} <+> switchm0))
-                   (switchmLst0 := fromSwitch0).
-            apply Bag.in_union in H0.
-            simpl in H0.
-            inversion HFMS; subst.
-            { destruct H0 as [[H0 | H0] | H0]; 
-              [idtac | solve[inversion H0] | idtac].
-              + inversion H0; subst.
-                eapply MkFMS...
-              + destruct (allFMS1 (Switch of_to0 pts1 tbl1 inp1 outp1 ctrlm1 switchm1)) as  [lnk [J [J0 J1]]]...
-                { apply Bag.in_union. right... }
-                destruct lnk; subst.
-                simpl in *.
-                subst.
-                assert (OpenFlowLink of_to0 fromSwitch0 fromCtrl = 
-                        OpenFlowLink of_to0 of_switchm0 of_ctrlm0) as X.
-                { eapply AllDiff_uniq... }
-                inversion X; subst; clear X.
-                
-                eapply FMS_untouched... }
-          + apply Bag.in_union in H0. simpl in H0.
-            destruct H0 as [[H0 | H0] | H0].
-            inversion H0; subst.
-            contradiction n...
-            inversion H0.
-            destruct (allFMS1 (Switch swId1 pts1 tbl1 inp1 outp1 ctrlm1
-                                      switchm1)) as [lnk [J [J0 J1]]]...
-            { apply Bag.in_union. right... }
-            exists lnk...
-            split...
-            apply in_app_iff in J. simpl in J.
-            destruct J as [J | [J | J]]...
-            simpl in J0.
-            destruct lnk.
-            simpl in J0.
-            subst.
-            inversion J; subst.
-            contradiction n... }
-        eexists...
-        eexists. eapply AllDiff_preservation. exact uniqOfLinkIds1.
-          simpl. do 2 rewrite -> map_app...
-        eexists. simpl. eauto.
-        eauto.
-        eauto.
-        eexists...
+        { eapply AllDiff_preservation.
+          exact uniqOfLinkIds1.
+          do 2 rewrite -> map_app... }
+        eexists. sauto.
+        eexists. sauto.
+        eexists. sauto.
+        sauto.
       (* Case 11. *)
-      + simpl in *.
-        exists (FlowTablesSafe_untouched tblsOk1).
-        exists linksTopoOk1.
-        exists (LinksHaveSrc_untouched haveSrc1).
-        exists (LinksHaveDst_untouched haveDst1).
-        exists (UniqSwIds_pres uniqSwIds1).
+      + eexists. sauto.
+        eexists. sauto.
+        eexists. sauto.
+        eexists. sauto.
+        eexists. sauto.
+        eexists. sauto.
         eexists.
-        unfold AllFMS in *. intros. destruct sw. subst.
-        assert ({swId0 = swId1 } + { swId0 <> swId1 }) as HIdEq.
-        { apply TotalOrder.eqdec. }
-        { destruct HIdEq; subst.
-          + exists (OpenFlowLink swId1 fromSwitch0 fromCtrl).
-            split...
-            split...
-            unfold UniqSwIds in uniqSwIds1.
-            assert (AllDiff swId (to_list 
-                                    (({| Switch swId1 pts0 tbl0 inp0 outp0 ({||}) 
-                                                ({|BarrierReply xid|} <+> switchm0)|}) <+> sws))) as uniqSwIds2.
-            { eapply Bag.AllDiff_preservation... }
-            assert (Switch swId1 pts0 tbl0 inp0 outp0 ({||}) ({|BarrierReply xid|} <+> switchm0) =
-                    Switch swId1 pts1 tbl1 inp1 outp1 ctrlm0 switchm1).
-            { eapply AllDiff_uniq. exact uniqSwIds2.
-              apply Bag.in_union.  left. simpl...
-              exact H0. simpl... }
-            inversion H1; subst; clear H1.
-            destruct (allFMS1 (Switch swId1 pts1 tbl1 inp1 outp1 ({||}) switchm0)) as [lnk [HLnkIn [HId HFMS]]].
-            { apply Bag.in_union. left. simpl. left. trivial. }
-            destruct lnk.
-            simpl in *.
-            subst.
-            assert (OpenFlowLink swId1 of_switchm0 of_ctrlm0 =
-                    OpenFlowLink swId1 fromSwitch0 (fromCtrl ++ [BarrierRequest xid])) as HEqOf.
-            { eapply AllDiff_uniq... }
-            inversion HEqOf; subst; clear HEqOf.
-            inversion HFMS; subst.
-            destruct H11 as [ctrlEp HSafeWire].
-            destruct (SafeWire_dequeue_BarrierRequest _ _ HSafeWire) as [switchEp2 [HSafeWire2 HEpEq]].
-            inversion H3; subst.
-            * apply MkFMS with (switchEp := switchEp2)...
-              apply NoFlowModsInBuffer. intros. simpl in H1. inversion H1.
-              auto.
-            *  inversion H11.
-               destruct ctrlm1.
-               rename to_list into lst.
-               unfold to_list in H2.
-               simpl in H2. 
-               rewrite <- OrderedLists.union_singleton_l in H2...
-               symmetry in H2.
-               apply OrderedLists.insert_nonempty in H2...
-               inversion H2.
-          + apply Bag.in_union in H0.
-            destruct H0.
-            simpl in H0.
-            destruct H0.
-            inversion H0; subst. contradiction n... inversion H0.
-            destruct (allFMS1 (Switch swId1 pts1 tbl1 inp1 outp1 
-                                      ctrlm0 switchm1)) 
-              as [lnk [HLnkIn [HId HFMS]]].
-            { apply Bag.in_union. right... }
-            exists lnk.
-            apply in_app_iff in HLnkIn.
-            simpl in HLnkIn.
-            { destruct HLnkIn as [HLnkIn | [HLnkIn | HLnkIn]].
-              + split...
-              + destruct lnk. inversion HLnkIn. contradiction n. subst...
-              + split... } }
-        exists...
-        exists. eapply AllDiff_preservation. exact uniqOfLinkIds1.
-          simpl. do 2 rewrite -> map_app...
-        exists. simpl. eauto.
-        eauto.
-        eexists...
-      (* Case 12. *)
-      + simpl in *.
-        exists (FlowTablesSafe_untouched tblsOk1).
-        exists linksTopoOk1.
-        exists (LinksHaveSrc_untouched haveSrc1).
-        exists (LinksHaveDst_untouched haveDst1).
-        exists (UniqSwIds_pres uniqSwIds1).
+        { eapply AllDiff_preservation.
+          exact uniqOfLinkIds1.
+          do 2 rewrite -> map_app... }
+        eexists. sauto.
+        eexists. sauto.
+        eexists. sauto.
+        sauto.
+      + eexists. sauto.
+        eexists. sauto.
+        eexists. sauto.
+        eexists. sauto.
+        eexists. sauto.
+        eexists. sauto.
         eexists.
-        unfold AllFMS in *. intros. destruct sw. subst.
-        assert ({swId0 = swId1 } + { swId0 <> swId1 }) as HIdEq.
-        { apply TotalOrder.eqdec. }
-        { destruct HIdEq; subst.
-          + exists (OpenFlowLink swId1 fromSwitch0 fromCtrl).
-            split...
-            split...
-            unfold UniqSwIds in uniqSwIds1.
-            destruct (allFMS1 (Switch swId1 pts0 tbl0 inp0 outp0 ctrlm0 switchm0)) as [lnk [HLnkIn [HId HFMS]]].
-            { apply Bag.in_union. left. simpl... }
-            simpl in *.
-            destruct lnk.
-            simpl in *.
-            subst.
-            assert (OpenFlowLink swId1 of_switchm0 of_ctrlm0 =
-                    OpenFlowLink swId1 fromSwitch0 (fromCtrl ++ [msg])) as HOfEq.
-            { eapply AllDiff_uniq... }
-            inversion HOfEq; subst; clear HOfEq.
-            assert (AllDiff swId 
-                      (to_list (({|Switch swId1 pts0 tbl0 inp0 outp0 ({|msg|}<+>ctrlm0) switchm0|}) <+> sws))).
-            { eapply Bag.AllDiff_preservation. exact uniqSwIds1. simpl... }
-            assert (Switch swId1 pts1 tbl1 inp1 outp1 ctrlm1 switchm1 = 
-                    Switch swId1 pts0 tbl0 inp0 outp0 ({|msg|}<+>ctrlm0) switchm0).
-            { 
-              eapply AllDiff_uniq.
-              exact H2. exact H1.
-              apply Bag.in_union. left. simpl...
-              simpl... }
-            inversion H3; subst; clear H3.
-            apply FMS_pop...
-          + apply Bag.in_union in H1.
-            destruct H1.
-            simpl in H1. destruct H1. inversion H1; subst; contradiction n...
-            inversion H1.
-            destruct (allFMS1 (Switch swId1 pts1 tbl1 inp1 outp1 ctrlm1 
-                                      switchm1)) as [lnk [HLnkIn [HId HFMS]]].
-            { apply Bag.in_union. right... }
-            exists lnk.
-            apply in_app_iff in HLnkIn.
-            simpl in HLnkIn.
-            { destruct HLnkIn as [HLnkIn | [HLnkIn | HLnkIn]].
-              + split...
-              + destruct lnk. inversion HLnkIn. contradiction n. subst...
-              + split... } }
-        eexists...
-        eexists. eapply AllDiff_preservation. exact uniqOfLinkIds1.
-          simpl. do 2 rewrite -> map_app...
-        eexists. simpl. eauto.
-        eauto.
-        eexists...
-    } 
+        { eapply AllDiff_preservation.
+          exact uniqOfLinkIds1.
+          do 2 rewrite -> map_app... }
+        eexists. sauto.
+        eexists. sauto.
+        eexists. sauto.
+        sauto.
     (* epic fail of a proof script *)
-    Grab Existential Variables. eauto. eauto. eauto. eauto. eauto. eauto. eauto. eauto. eauto. eauto. eauto. eauto.
-    eauto. eauto. eauto. eauto. eauto. eauto. eauto. eauto. eauto. eauto.
+    Grab Existential Variables. 
+    eauto. eauto. eauto. eauto. eauto. eauto. eauto. 
+    eauto. eauto. eauto. eauto. eauto. eauto. eauto. 
+    eauto. eauto. eauto. eauto. eauto. eauto. eauto. 
+    eauto. eauto. eauto. eauto. eauto. eauto. eauto. 
+    eauto. eauto. eauto. eauto. eauto. eauto. eauto. 
+    eauto. eauto. 
+    }
   Qed.
 
   Lemma simpl_multistep' : forall (st1 st2 : state) obs
@@ -1208,22 +241,21 @@ Module Make (AtomsAndController_ : ATOMS_AND_CONTROLLER) <: RELATION.
     (haveSrc1 : LinksHaveSrc (switches st1) (links st1))
     (haveDst1 : LinksHaveDst (switches st1) (links st1))
     (uniqSwIds1 : UniqSwIds (switches st1))
-    (allFMS1 : AllFMS (switches st1) (ofLinks st1))
     (P1 : P (switches st1) (ofLinks st1) (ctrl st1))
     (uniqOfLinkIds1 : AllDiff of_to (ofLinks st1))
     (ofLinksHaveSw1 : OFLinksHaveSw (switches st1) (ofLinks st1))
     (devsFromTopo1 : DevicesFromTopo st1)
-    (swsHaveOFLinks1 : SwitchesHaveOpenFlowLinks st1),
+    (swsHaveOFLinks1 : SwitchesHaveOpenFlowLinks (switches st1) (ofLinks st1)),
     multistep step st1 obs st2 ->
-    exists tblsOk2 linksTopoOk2 haveSrc2 haveDst2 uniqSwIds2 allFMS2 P2
+    exists tblsOk2 linksTopoOk2 haveSrc2 haveDst2 uniqSwIds2 P2
            uniqOfLinkIds2 ofLinksHaveSw2 devsFromTopo2 swsHaveOFLinks2,
       multistep concreteStep
                 (ConcreteState st1 tblsOk1 linksTopoOk1 haveSrc1 haveDst1 
-                               uniqSwIds1 allFMS1 P1 uniqOfLinkIds1
+                               uniqSwIds1 P1 uniqOfLinkIds1
                                ofLinksHaveSw1 devsFromTopo1 swsHaveOFLinks1)
                 obs
                 (ConcreteState st2 tblsOk2 linksTopoOk2 haveSrc2 haveDst2 
-                               uniqSwIds2 allFMS2 P2 uniqOfLinkIds2
+                               uniqSwIds2 P2 uniqOfLinkIds2
                                ofLinksHaveSw2 devsFromTopo2 swsHaveOFLinks2).
   Proof with eauto with datatypes.
     intros.
@@ -1232,32 +264,32 @@ Module Make (AtomsAndController_ : ATOMS_AND_CONTROLLER) <: RELATION.
     + solve [ eauto 12 ].
     (* tau step *)
     + destruct (simpl_step tblsOk1 linksTopoOk1 haveSrc1 haveDst1 
-                           uniqSwIds1 allFMS1 P1 uniqOfLinkIds1 ofLinksHaveSw1
+                           uniqSwIds1 P1 uniqOfLinkIds1 ofLinksHaveSw1
                            devsFromTopo1 swsHaveOFLinks1 H)
         as [tblsOk2 [linksTopoOk2 [haveSrc2 [haveDst2 [uniqSwIds2 
-                [allFMS2 [P2 [uniqOfLinkIds2 [ofLinksHaveSw2 
-           [devsFromTopo2 [swsHaveOFLinks2 step]]]]]]]]]]].
+           [P2 [uniqOfLinkIds2 [ofLinksHaveSw2 
+           [devsFromTopo2 [swsHaveOFLinks2 step]]]]]]]]]].
       destruct (IHmultistep tblsOk2 linksTopoOk2 haveSrc2 haveDst2 
-                            uniqSwIds2 allFMS2 P2 uniqOfLinkIds2 ofLinksHaveSw2
+                            uniqSwIds2 P2 uniqOfLinkIds2 ofLinksHaveSw2
                             devsFromTopo2 swsHaveOFLinks2)
         as [tblsOk3 [linksTopoOk3 [haveSrc3 [haveDst3
-                [uniqSwIds3 [allFMS3 [PN [uniqOfLinkIdsN [ofLinksHaveSwN 
-           [devsFromTopoN [swsHaveOFLinksN stepN]]]]]]]]]]].
-      solve [ eauto 13 ].
+                [uniqSwIds3 [PN [uniqOfLinkIdsN [ofLinksHaveSwN 
+           [devsFromTopoN [swsHaveOFLinksN stepN]]]]]]]]]].
+      solve [ eauto 12 ].
     (* The script below is an identical copy of the case above. *)
     + destruct (simpl_step tblsOk1 linksTopoOk1 haveSrc1 haveDst1 
-                           uniqSwIds1 allFMS1 P1 uniqOfLinkIds1 ofLinksHaveSw1
+                           uniqSwIds1 P1 uniqOfLinkIds1 ofLinksHaveSw1
                            devsFromTopo1 swsHaveOFLinks1 H)
         as [tblsOk2 [linksTopoOk2 [haveSrc2 [haveDst2 [uniqSwIds2 
-                [allFMS2 [P2 [uniqOfLinkIds2 [ofLinksHaveSw2 
-           [devsFromTopo2 [swsHaveOFLinks2 step]]]]]]]]]]].
+           [P2 [uniqOfLinkIds2 [ofLinksHaveSw2 
+           [devsFromTopo2 [swsHaveOFLinks2 step]]]]]]]]]].
       destruct (IHmultistep tblsOk2 linksTopoOk2 haveSrc2 haveDst2 
-                            uniqSwIds2 allFMS2 P2 uniqOfLinkIds2 ofLinksHaveSw2
+                            uniqSwIds2 P2 uniqOfLinkIds2 ofLinksHaveSw2
                             devsFromTopo2 swsHaveOFLinks2)
         as [tblsOk3 [linksTopoOk3 [haveSrc3 [haveDst3
-                [uniqSwIds3 [allFMS3 [PN [uniqOfLinkIdsN [ofLinksHaveSwN 
-           [devsFromTopoN [swsHaveOFLinksN stepN]]]]]]]]]]].
-      solve [ eauto 13 ].
+                [uniqSwIds3 [PN [uniqOfLinkIdsN [ofLinksHaveSwN 
+           [devsFromTopoN [swsHaveOFLinksN stepN]]]]]]]]]].
+      solve [ eauto 12 ].
   Qed.
 
   Lemma simpl_multistep : forall (st1 : concreteState) (devs2 : state) obs,
@@ -1270,9 +302,9 @@ Module Make (AtomsAndController_ : ATOMS_AND_CONTROLLER) <: RELATION.
     destruct st1.
     destruct (simpl_multistep' concreteState_flowTableSafety0
       concreteState_consistentDataLinks0 linksHaveSrc0 linksHaveDst0
-      uniqSwIds0 allFMS0 ctrlP0 uniqOfLinkIds0 ofLinksHaveSw0 devicesFromTopo0
-      swsHaveOFLinks0 H) as [v0 [v1 [v2 [v3 [v4 [v5 [v6 [v7 [v8 [v9 [v10 Hstep]]]]]]]]]]].
-    exists (ConcreteState devs2 v0 v1 v2 v3 v4 v5 v6 v7 v8 v9 v10)...
+      uniqSwIds0 ctrlP0 uniqOfLinkIds0 ofLinksHaveSw0 devicesFromTopo0
+      swsHaveOFLinks0 H) as [v0 [v1 [v2 [v3 [v4 [v5 [v6 [v7 [v8 [v9 Hstep]]]]]]]]]].
+    exists (ConcreteState devs2 v0 v1 v2 v3 v4 v5 v6 v7 v8 v9)...
   Qed.
 
   Lemma relate_step_simpl_tau : forall st1 st2,
@@ -1394,16 +426,15 @@ Module Make (AtomsAndController_ : ATOMS_AND_CONTROLLER) <: RELATION.
     destruct devices1.
     subst.
     simpl in *.
-    inversion H1. subst. clear H1.
-    inversion H6. subst. clear H6.
-
+    inversion H1; subst; clear H1.
+    inversion H6; subst; clear H6.
     assert (FlowTableSafe sw tbl0) as Z.
-      unfold FlowTablesSafe in concreteState_flowTableSafety0.
-      eapply concreteState_flowTableSafety0...
-      apply Bag.in_union.
-      left.
-      simpl...
-    unfold FlowTableSafe in Z.
+    { assert (FlowModSafe sw tbl0 ctrlm0) as Z.
+      { unfold FlowTablesSafe in concreteState_flowTableSafety0.
+        eapply concreteState_flowTableSafety0...
+        apply Bag.in_union; simpl... }
+      unfold FlowTableSafe in Z.
+      inversion Z... }
     remember (Z pt pk outp' pksToCtrl H3) as Y eqn:X. clear X Z.
     rewrite <- Y. clear Y.
 
