coq/FwOF/FwOFBisimulation.v
@@ -3,6 +3,7 @@ Set Implicit Arguments.
 Require Import Coq.Classes.Equivalence.
 Require Import Common.Bisimulation.
 Require Import FwOF.FwOFSignatures.
+Require FwOF.FwOFRelationDefinitions.
 Require FwOF.FwOFWellFormedness.
 Require FwOF.FwOFWeakSimulation1.
 Require FwOF.FwOFWeakSimulation2.
@@ -11,11 +12,13 @@ Local Open Scope equiv_scope.
 
 Module Make (AtomsAndController : ATOMS_AND_CONTROLLER).
 
-  Module WellFormedness := FwOF.FwOFWellFormedness.Make (AtomsAndController).
-  Module WeakSim1 := FwOF.FwOFWeakSimulation1.Make (WellFormedness).
-  Module WeakSim2 := FwOF.FwOFWeakSimulation2.Make (WellFormedness).
+  Module RelationDefinitions := FwOF.FwOFRelationDefinitions.Make (AtomsAndController).
+  Module Relation := FwOF.FwOFWellFormedness.Make (RelationDefinitions).
+  Module WeakSim1 := FwOF.FwOFWeakSimulation1.Make (RelationDefinitions).
+  Module WeakSim2 := FwOF.FwOFWeakSimulation2.Make (Relation).
 
-  Import WellFormedness.
+  Import Relation.
+  Import RelationDefinitions.
 
   Theorem fwof_abst_weak_bisim :
     weak_bisimulation concreteStep abstractStep bisim_relation.
