coq/FwOF/FwOFWellFormednessLemmas.v
@@ -1,0 +1,577 @@
+Set Implicit Arguments.
+
+Require Import Coq.Lists.List.
+Require Import Common.Types.
+Require Import Common.Bisimulation.
+Require Import Common.AllDiff.
+Require Import Bag.Bag2.
+Require Import FwOF.FwOFSignatures.
+
+Local Open Scope list_scope.
+Local Open Scope bag_scope.
+
+Module Make (Import RelationDefinitions : RELATION_DEFINITIONS).
+
+  Import AtomsAndController.
+  Import Machine.
+  Import Atoms.
+
+  Lemma LinksHaveSrc_untouched : forall 
+    {swId tbl pts sws links
+    inp outp ctrlm switchm tbl' inp' outp' ctrlm' switchm' },
+    LinksHaveSrc 
+      ({| Switch swId pts tbl inp outp ctrlm switchm |} <+> sws)  links ->
+    LinksHaveSrc 
+      ({| Switch swId pts tbl' inp' outp' ctrlm' switchm' |} <+> sws)
+      links.
+  Proof with auto.
+    intros.
+    unfold LinksHaveSrc in *.
+    intros.
+    apply H in H0. clear H.
+    unfold LinkHasSrc in *.
+    destruct H0 as [sw [HMem [HEq HIn]]].
+    simpl in HMem.
+    rewrite -> Bag.in_union in HMem.
+    destruct HMem.
+    + destruct sw.
+      simpl in *.
+      destruct H.
+      inversion H.
+      subst.
+      eexists.
+      split. 
+      apply Bag.in_union. left. simpl. left. reflexivity.
+      simpl...
+      inversion H.
+    + exists sw.
+      split...
+      simpl...
+      apply Bag.in_union...
+  Qed.
+
+  Lemma LinksHaveDst_untouched : forall 
+    {swId tbl pts sws links
+    inp outp ctrlm switchm tbl' inp' outp' ctrlm' switchm' },
+    LinksHaveDst
+      ({| Switch swId pts tbl inp outp ctrlm switchm |} <+>  sws)  links ->
+    LinksHaveDst 
+      ({| Switch swId pts tbl' inp' outp' ctrlm' switchm' |} <+> sws)
+      links.
+  Proof with auto.
+
+    intros.
+    unfold LinksHaveDst in *.
+    intros.
+    apply H in H0. clear H.
+    unfold LinkHasDst in *.
+    destruct H0 as [sw [HMem [HEq HIn]]].
+    simpl in HMem.
+    rewrite -> Bag.in_union in HMem.
+    destruct HMem.
+    + destruct sw.
+      simpl in *.
+      destruct H.
+      inversion H.
+      subst.
+      eexists.
+      split. 
+      apply Bag.in_union. left. simpl. left. reflexivity.
+      simpl...
+      inversion H.
+    + exists sw.
+      split...
+      simpl...
+      apply Bag.in_union...
+  Qed.
+
+   Lemma LinkTopoOK_inv : forall {links links0 src dst} pks pks',
+     ConsistentDataLinks (links ++ (DataLink src pks dst) :: links0) ->
+     ConsistentDataLinks (links ++ (DataLink src pks' dst) :: links0).
+   Proof with auto with datatypes.
+     intros.
+     unfold ConsistentDataLinks in *.
+     intros.
+     apply in_app_iff in H0.
+     simpl in H0.
+     destruct H0 as [H0 | [H0 | H0]]...
+     pose (lnk' := (DataLink src0 pks0 dst0)).
+     remember (H lnk').
+     assert (In lnk' (links0 ++ lnk' :: links1))...
+     apply e in H1.
+     simpl in H1.
+     inversion H0.
+     simpl...
+   Qed.
+
+
+  Lemma FlowTablesSafe_untouched : forall {sws swId pts tbl inp inp'
+    outp outp' ctrlm switchm switchm' },
+    FlowTablesSafe
+      ({|Switch swId pts tbl inp outp ctrlm switchm|} <+> sws) ->
+    FlowTablesSafe 
+      ({|Switch swId pts tbl inp' outp' ctrlm switchm'|} <+> sws).
+  Proof with eauto.
+    intros.
+    unfold FlowTablesSafe in *.
+    intros.
+    simpl in H0.
+    apply Bag.in_union in H0; simpl in H0.
+    destruct H0 as [[H0 | H0] | H0].
+    + inversion H0; subst; clear H0.
+      eapply H...
+      apply Bag.in_union; simpl...
+    + inversion H0.
+    + eapply H.
+      apply Bag.in_union...
+  Qed.
+
+  Lemma FlowModSafe_PacketOut : forall swId tbl pt pk ctrlm,
+    FlowModSafe swId tbl (({|PacketOut pt pk|}) <+> ctrlm) ->
+    FlowModSafe swId tbl ctrlm.
+  Proof with eauto.
+    intros.
+    inversion H; subst.
+    + apply NoFlowModsInBuffer...
+      intros. apply H0. apply Bag.in_union...
+    + remember (Bag2Lemmas.union_from_ordered _ _ _ _ _ H0) as J0 eqn:X; clear X.
+      clear H0.
+      assert (In (FlowMod f) (to_list ctrlm0)) as X.
+      { assert (In (FlowMod f) (to_list (({|PacketOut pt pk|}) <+> ctrlm0))).
+        { rewrite <- J0.
+          rewrite -> Bag.in_union; simpl... }
+        rewrite -> Bag.in_union in H0.
+        simpl in H0; destruct H0 as [[H0|H0]|H0]; solve [auto;inversion H0]. }
+      apply Bag.in_split with (Order:=TotalOrder_fromController) in X.
+      destruct X as [rest Heq].
+      subst.
+      eapply OneFlowModsInBuffer...
+      intros.
+      rewrite <- Bag.union_assoc in J0.
+      rewrite -> (Bag.union_comm _ ({|PacketOut pt pk|})) in J0.
+      rewrite -> Bag.union_assoc in J0.
+      apply Bag.pop_union_l in J0.
+      subst.
+      apply H1...
+      apply Bag.in_union...
+  Qed.
+
+  Lemma FlowTablesSafe_PacketOut : forall sws swId pts tbl inp inp'
+    outp outp' ctrlm switchm switchm' pt pk,
+    FlowTablesSafe
+      ({|Switch swId pts tbl inp outp (({|PacketOut pt pk|}) <+> ctrlm) switchm|} <+> sws) ->
+    FlowTablesSafe 
+      ({|Switch swId pts tbl inp' outp' ctrlm switchm'|} <+> sws).
+  Proof with eauto.
+    intros.
+    unfold FlowTablesSafe in *.
+    intros.
+    simpl in H0.
+    apply Bag.in_union in H0; simpl in H0.
+    destruct H0 as [[H0 | H0] | H0].
+    + inversion H0; subst; clear H0.
+      assert (FlowModSafe swId1 tbl1 (({|PacketOut pt pk|} <+> ctrlm1))) as X.
+      { eapply H...
+        apply Bag.in_union; simpl... }
+      eapply FlowModSafe_PacketOut...
+    + inversion H0.
+    + eapply H. apply Bag.in_union. right...
+  Qed.
+
+  Lemma LinksHaveSrc_inv : forall {sws links links0 src dst} pks pks',
+    LinksHaveSrc sws (links ++ (DataLink src pks dst) :: links0) ->
+    LinksHaveSrc sws (links ++ (DataLink src pks' dst) :: links0).
+  Proof with auto with datatypes.
+    intros.
+    unfold LinksHaveSrc in *.
+    intros.
+    apply in_app_iff in H0.
+    simpl in H0.
+    destruct H0 as [H0 | [H0 | H0]]; subst...
+    destruct (H (DataLink src0 pks0 dst0))...
+    destruct H0 as [HMem [HEq HIn]].
+    simpl in *.
+    unfold LinkHasSrc.
+    exists x...
+  Qed.
+
+  Lemma LinksHaveDst_inv : forall {sws links links0 src dst} pks pks',
+    LinksHaveDst sws (links ++ (DataLink src pks dst) :: links0) ->
+    LinksHaveDst sws (links ++ (DataLink src pks' dst) :: links0).
+  Proof with auto with datatypes.
+    intros.
+    unfold LinksHaveDst in *.
+    intros.
+    apply in_app_iff in H0.
+    simpl in H0.
+    destruct H0 as [H0 | [H0 | H0]]; subst...
+    destruct (H (DataLink src0 pks0 dst0))...
+    destruct H0 as [HMem [HEq HIn]].
+    simpl in *.
+    unfold LinkHasDst.
+    exists x...
+  Qed.
+
+  Lemma UniqSwIds_pres : forall {sws swId pts tbl inp outp ctrlm switchm
+    pts' tbl' inp' outp' ctrlm' switchm'},
+    UniqSwIds ({|Switch swId pts tbl inp outp ctrlm switchm|} <+> sws) ->
+    UniqSwIds ({|Switch swId pts' tbl' inp' outp' ctrlm' switchm'|} <+> sws).
+  Proof with auto with datatypes.
+    intros.
+    unfold UniqSwIds in *.
+    unfold union in H.
+    unfold to_list in H.
+    simpl in H.
+    destruct sws.
+    rename to_list into swsLst.
+    unfold union.
+    unfold to_list.
+    simpl.
+    (* might need induction (shouldn't since swId is the same *)
+  Admitted.
+
+  Lemma OfLinksHaveSrc_pres1 : forall { sws swId pts1 tbl1 inp1 outp1 ctrlm1 
+    switchm1 pts2 tbl2 inp2 outp2 ctrlm2 switchm2 switchmLst1 ctrlmLst1
+    switchmLst2 ctrlmLst2 ofLinks1 ofLinks2 },
+    OFLinksHaveSw
+      ({|Switch swId pts1 tbl1 inp1 outp1 ctrlm1 switchm1|} <+> sws)
+      (ofLinks1 ++ OpenFlowLink swId switchmLst1 ctrlmLst1 :: ofLinks2) ->
+    OFLinksHaveSw
+      ({|Switch swId pts2 tbl2 inp2 outp2 ctrlm2 switchm2|} <+> sws)
+      (ofLinks1 ++ OpenFlowLink swId switchmLst2 ctrlmLst2 :: ofLinks2).
+  Proof with auto with datatypes.
+    intros.
+    unfold OFLinksHaveSw in *.
+    intros.
+    destruct ofLink.
+    unfold ofLinkHasSw in *.
+    apply in_app_iff in H0; simpl in H0; destruct H0 as [H0 | [H0 | H0]]; subst.
+    + destruct H with (ofLink := OpenFlowLink of_to0 of_switchm0 of_ctrlm0)
+        as [sw [HMem HEq]]...
+      assert ({ of_to0 = swId0 } + { of_to0 <> swId0 }) as J by (apply TotalOrder.eqdec).
+      destruct J; subst.
+      - exists (Switch swId0 pts2 tbl2 inp2 outp2 ctrlm2 switchm2).
+        split...
+        apply Bag.in_union.
+        left.
+        simpl...
+      - exists sw.
+        destruct sw.
+        simpl in HEq.
+        subst.
+        split...
+        apply Bag.in_union.
+        right.
+        apply Bag.in_union in HMem.
+        destruct HMem.
+        * simpl in H1.
+          destruct H1.
+          inversion H1.
+          subst.
+          contradiction n...
+          inversion H1.
+        * trivial.
+    + inversion H0; subst; clear H0.
+      exists (Switch of_to0 pts2 tbl2 inp2 outp2 ctrlm2 switchm2).
+      split...
+      apply Bag.in_union.
+      left.
+      simpl...
+    + destruct H with (ofLink := OpenFlowLink of_to0 of_switchm0 of_ctrlm0) 
+        as [sw [HMem HEq]]...
+      assert ({ of_to0 = swId0 } + { of_to0 <> swId0 }) as J by (apply TotalOrder.eqdec).
+      destruct J; subst.
+      - exists (Switch swId0 pts2 tbl2 inp2 outp2 ctrlm2 switchm2).
+        split... apply Bag.in_union. left. simpl...
+      - exists sw.
+        destruct sw.
+        simpl in HEq.
+        subst.
+        split...
+        apply Bag.in_union.
+        right.
+        apply Bag.in_union in HMem.
+        destruct HMem...
+        simpl in H1.
+        destruct H1.
+        * inversion H1.
+          subst.
+          contradiction n...
+        * inversion H1.
+  Qed.
+
+  Lemma OfLinksHaveSrc_pres2 : forall { sws swId pts1 tbl1 inp1 outp1 ctrlm1 
+    switchm1 pts2 tbl2 inp2 outp2 ctrlm2 switchm2 ofLinks },
+    OFLinksHaveSw
+      ({|Switch swId pts1 tbl1 inp1 outp1 ctrlm1 switchm1|} <+> sws)
+      ofLinks ->
+    OFLinksHaveSw
+      ({|Switch swId pts2 tbl2 inp2 outp2 ctrlm2 switchm2|} <+> sws)
+      ofLinks.
+  Proof with auto with datatypes.
+    intros.
+    unfold OFLinksHaveSw in *.
+    intros.
+    destruct ofLink.
+    apply H in H0.
+    clear H.
+    unfold ofLinkHasSw in *.
+    destruct H0 as [sw [HMem HEq]].
+    simpl in HEq.
+    destruct sw.
+    assert ({ of_to0 = swId0 } + { of_to0 <> swId0 }) as J by (apply TotalOrder.eqdec).
+    destruct J; subst.
+    simpl in *. subst.
+    exists (Switch swId0 pts2 tbl2 inp2 outp2 ctrlm2 switchm2).
+    split... 
+    + apply Bag.in_union.
+      left.
+      simpl...
+    + exists (Switch swId1 pts0 tbl0 inp0 outp0 ctrlm0 switchm0).
+      apply Bag.in_union in HMem.
+      destruct HMem.
+      - simpl in H.
+        destruct H.
+        * inversion H.
+          subst.
+          simpl in n.
+          contradiction n...
+        * inversion H.
+      - split...
+        apply Bag.in_union...
+  Qed.
+
+  Lemma OfLinksHaveSrc_pres3 : forall { sws swId switchmLst1 ctrlmLst1
+    switchmLst2 ctrlmLst2 ofLinks1 ofLinks2 },
+    OFLinksHaveSw sws
+      (ofLinks1 ++ OpenFlowLink swId switchmLst1 ctrlmLst1 :: ofLinks2) ->
+    OFLinksHaveSw sws
+      (ofLinks1 ++ OpenFlowLink swId switchmLst2 ctrlmLst2 :: ofLinks2).
+  Proof with auto with datatypes.
+    intros.
+    unfold OFLinksHaveSw in *.
+    intros.
+    destruct ofLink.
+    apply in_app_iff in H0; simpl in H0; destruct H0 as [H0 | [H0 | H0]]; subst...
+    inversion H0; subst; clear H0.
+    unfold ofLinkHasSw in *.
+    destruct (H (OpenFlowLink of_to0 switchmLst1 ctrlmLst1)) as [sw [HMem HEq]]...
+    exists sw...
+  Qed.
+
+  Hint Resolve OfLinksHaveSrc_pres1 OfLinksHaveSrc_pres2 OfLinksHaveSrc_pres3.
+
+  Hint Unfold UniqSwIds.
+  Hint Resolve P_entails_FlowTablesSafe.
+
+  Section DevicesFromTopo.
+    
+    Hint Unfold DevicesFromTopo.
+
+    Lemma DevicesFromTopo_pres0 : forall swId0 pts0 tbl0 inp0 outp0 ctrlm0
+      switchm0 pts1 tbl1 inp1 outp1 ctrlm1 switchm1 sws links0 ofLinks0
+      ctrl0,
+      DevicesFromTopo
+        (State ({|Switch swId0 pts0 tbl0 inp0 outp0 ctrlm0 switchm0|} <+> sws)
+               links0
+               ofLinks0
+               ctrl0) ->
+      DevicesFromTopo
+        (State ({|Switch swId0 pts1 tbl1 inp1 outp1 ctrlm1 switchm1|} <+> sws)
+               links0
+               ofLinks0
+               ctrl0).
+    Proof with simpl; eauto.
+      intros.
+      unfold DevicesFromTopo in *.
+      intros.
+      apply H in H0.
+      clear H.
+      destruct H0 as [sw0 [sw1 [lnk [HMemSw0 [HMemSw1 [HInLnk [HSw0Eq [HSw1Eq
+                     [HLnkSrcEq HLnkDstEq]]]]]]]]].
+      destruct lnk.
+      simpl in *.
+      destruct sw0.
+      destruct sw1.
+      simpl in *.
+      subst.
+      apply Bag.in_union in HMemSw0.
+      apply Bag.in_union in HMemSw1.
+      destruct HMemSw0; destruct HMemSw1.
+      + eexists. eexists. eexists.
+        simpl in H; simpl in H0.
+        destruct H0; destruct H...
+        inversion H; inversion H0...
+        subst...
+        subst...
+        split...
+        apply Bag.in_union.
+        left...
+        split...
+        apply  Bag.in_union. left...
+        split...
+        inversion H.
+        inversion H0.
+        inversion H.
+      + do 3 eexists.
+        simpl in H.
+        destruct H. 2: solve[inversion H].
+        inversion H. subst.
+        repeat split.
+        apply Bag.in_union. left. simpl. left. reflexivity.
+        apply Bag.in_union. right. exact H0.
+        exact HInLnk.
+        trivial.
+        trivial.
+        trivial.
+        trivial.
+      + do 3 eexists.
+        simpl in H0.
+        destruct H0. 2: solve[inversion H0].
+        inversion H0; subst; clear H0.
+        repeat split...
+        apply Bag.in_union. right. exact H.
+        apply Bag.in_union. left. simpl. left. reflexivity.
+        trivial.
+        trivial.
+      + do 3 eexists.
+        repeat split...
+        apply Bag.in_union. right. exact H.
+        apply Bag.in_union. right. exact H0.
+        trivial.
+        trivial.
+    Qed.
+
+    Lemma DevicesFromTopo_pres1 : forall sws0 links0 links1 src
+      dst pks0 pks1 ofLinks0 ctrl0,
+      DevicesFromTopo
+        (State sws0
+               (links0 ++ DataLink src pks0 dst :: links1)
+               ofLinks0
+               ctrl0) ->
+      DevicesFromTopo
+        (State sws0
+               (links0 ++ DataLink src pks1 dst :: links1)
+               ofLinks0
+               ctrl0).
+    Proof with simpl; eauto with datatypes.
+      intros.
+      unfold DevicesFromTopo in *.
+      intros.
+      apply H in H0.
+      clear H.
+      destruct H0 as [sw0 [sw1 [lnk [HMemSw0 [HMemSw1 [HInLnk [HSw0Eq [HSw1Eq
+                     [HLnkSrcEq HLnkDstEq]]]]]]]]].
+      destruct lnk.
+      simpl in *.
+      destruct sw0.
+      destruct sw1.
+      simpl in *.
+      subst.
+      rewrite -> in_app_iff in HInLnk. simpl in HInLnk.
+      destruct HInLnk as [HInLnk | [HInLnk | HInLnk]].
+      + repeat eexists.
+        exact HMemSw0.
+        exact HMemSw1.
+        instantiate (1 := DataLink (swId1,pt1) pks2 (swId0,pt0)).
+        auto with datatypes.
+        simpl...
+        simpl...
+        simpl...
+        simpl...
+      + repeat eexists.
+        exact HMemSw0.
+        exact HMemSw1.
+        instantiate (1 := DataLink (swId1,pt1) pks1 (swId0,pt0)).
+        inversion HInLnk. subst.
+        auto with datatypes.
+        simpl...
+        simpl...
+        simpl...
+        simpl...
+      + repeat eexists.
+        exact HMemSw0.
+        exact HMemSw1.
+        instantiate (1 := DataLink (swId1,pt1) pks2 (swId0,pt0)).
+        auto with datatypes.
+        simpl...
+        simpl...
+        simpl...
+        simpl...
+    Qed.
+        
+  End DevicesFromTopo.
+
+  Section SwitchesHaveOpenFlowLinks.
+    
+    Hint Unfold SwitchesHaveOpenFlowLinks.
+
+    Lemma SwitchesHaveOpenFlowLinks_pres0 : forall swId0 pts0 tbl0 inp0 outp0 
+      ctrlm0 switchm0 pts1 tbl1 inp1 outp1 ctrlm1 switchm1 sws ofLinks0,
+      SwitchesHaveOpenFlowLinks
+        ({|Switch swId0 pts0 tbl0 inp0 outp0 ctrlm0 switchm0|} <+> sws)
+        ofLinks0 ->
+      SwitchesHaveOpenFlowLinks
+        ({|Switch swId0 pts1 tbl1 inp1 outp1 ctrlm1 switchm1|} <+> sws)
+               ofLinks0.
+    Proof with simpl; eauto.
+      intros.
+      unfold SwitchesHaveOpenFlowLinks in *.
+      intros.
+      simpl in *.
+      apply Bag.in_union in H0.
+      simpl in H0.
+      destruct H0 as [[H0 | H0] | H0].
+      + destruct sw.
+        inversion H0; subst; clear H0.
+        apply H.
+        apply Bag.in_union.
+        (*
+      + assert ( (Switch swId0 pts0 tbl0 inp0 outp0 ctrlm0 switchm0)  === (Switch swId0 pts0 tbl0 inp0 outp0 ctrlm0 switchm0) \/ Mem (Switch swId0 pts0 tbl0 inp0 outp0 ctrlm0 switchm0) sws).
+        left. apply reflexivity.
+        apply H in H1. clear H.
+        destruct H1 as [ofLink [HIn HSwEq]].
+        destruct ofLink.
+        simpl in *.
+        subst.
+        inversion H0; subst.
+        eexists...
+      + destruct (H sw (or_intror H0)) as [ofLink [HIn HSwEq]].
+        destruct ofLink.
+        simpl in *.
+        subst.
+        destruct sw.
+        simpl in *.
+        subst.
+        eexists... *)
+    Admitted.
+
+    Lemma SwitchesHaveOpenFlowLinks_pres1 : forall sws0 ofLinks0
+      ofLinks1 swId switchm0 ctrlm0 switchm1 ctrlm1,
+      SwitchesHaveOpenFlowLinks
+        sws0
+        (ofLinks0 ++ OpenFlowLink swId switchm0 ctrlm0 :: ofLinks1) ->
+      SwitchesHaveOpenFlowLinks
+        sws0
+        (ofLinks0 ++ OpenFlowLink swId switchm1 ctrlm1 :: ofLinks1).
+      Proof with eauto with datatypes.
+        unfold SwitchesHaveOpenFlowLinks.
+        intros.
+        simpl in *.
+        apply H in H0.
+        clear H.
+        destruct H0 as [ofLink [HIn HIdEq]].
+        apply in_app_iff in HIn.
+        simpl in HIn.
+        destruct HIn as [HIn | [HIn | HIn]].
+        + eexists...
+        + exists (OpenFlowLink swId0 switchm1 ctrlm1).
+          split...
+          subst.
+          simpl in *...
+        + eexists...
+      Qed.
+        
+  End SwitchesHaveOpenFlowLinks.
+
+End Make.
